theories/L6_PCPS/shrink_cps_correct.v
@@ -1,13 +1,13 @@
 Require Import Coq.Relations.Relations.
-Require Import Coq.Relations.Relations.
 Require Import Coq.Setoids.Setoid.
 Require Import Coq.Classes.Morphisms.
 Import RelationClasses.
 
+
+Require compcert.lib.Maps.
 Require Import ExtLib.Data.Bool.
-
 Require Coq.funind.Recdef.
-
+Import Nnat.
 Require Import Coq.Arith.Arith Coq.NArith.BinNat ExtLib.Data.String ExtLib.Data.List Coq.omega.Omega Coq.Program.Program Coq.micromega.Psatz Coq.Sets.Ensembles Coq.Logic.Decidable Coq.Lists.ListDec.
 Require Import Libraries.CpdtTactics Coq.Sorting.Permutation.
 Require Import Libraries.HashMap.
@@ -15,21 +15,14 @@ Require Import Libraries.maps_util.
 Require Import compcert.lib.Coqlib L6.Ensembles_util. 
 Require Import L6.cps.
 Require Import L6.ctx L6.logical_relations.
-Require Import L6.cps_util L6.List_util L6.shrink_cps L6.eval L6.set_util L6.identifiers.
-Import Nnat.
+Require Import L6.cps_util L6.List_util L6.shrink_cps L6.eval L6.set_util L6.identifiers L6.stemctx.
+
    Ltac pi0 :=
     repeat match goal with
              | [ H: _ + _ = 0 |- _ ] =>  apply plus_is_O in H; destruct H; subst; pi0
              | [ H: 0 = _ + _ |- _ ] => symmetry in H; pi0
              | [ H: (if cps_util.var_dec ?X ?Y then _ else _) = 0 |- _] => destruct (cps_util.var_dec X Y); try inversion H; pi0                | [ H: ?X <> ?X |- _] => exfalso; apply H; auto
            end.
-
-
-
-
-
-
-
 
 
 
@@ -60,57 +53,69 @@ Proof.
   reflexivity.
 Qed.
 
+     Inductive unique_name_fundefs: fundefs -> Prop :=
+     | Uname_Fcons: forall f tau ys e defs,
+                      ~ name_in_fundefs defs f ->
+                      unique_name_fundefs defs ->
+                      unique_name_fundefs (Fcons f tau ys e defs)
+     | Uname_Fnil:
+         unique_name_fundefs Fnil
+     .
+
+
   (** general rewrite rules that preserves semantics
     - Fun_inline replaces one occurence on f by its definition
-    - Fun_dead removes the definition of a set of functions if none of them occur in the rest of the program
+    - Fun_dead removes the definition of a set of functions if none of them occur free in the rest of the program
     - Fun_rm removes a function if it doesn't occur anywhere in its mutual bundle or in the rest of the term
-    -  Constr_dead removes the binding of a datatype when it doesn't appear in the rest of the program 
+    -  Constr_dead removes the binding of a datatype when it doesn't occur free in the rest of the program 
     -  Constr_proj replaces a binding by the nth projection of a datatype when the datatype is known (in ctx) 
     -  Constr_case reduces a pattern match into an application of the right continuation on the datatype when the datatype is known
 *)
   Inductive rw: relation exp :=
   (* Rules about dead var elimination *)
 | Constr_dead: forall x t ys e, 
-                 num_occur e x 0 ->
+                 ~ occurs_free e x ->
                  rw (Econstr x t ys e) e
 | Prim_dead: forall x p ys e,
-               num_occur e x 0 ->
+               ~ occurs_free e x ->
                rw (Eprim x p ys e) e
 | Proj_dead: forall x t n y e,
-               num_occur e x 0 ->
+               ~ occurs_free e x ->
                rw (Eproj x t n y e) e
 | Fun_dead: forall e fds,
-              Forall (fun v => num_occur e v 0) (all_fun_name fds) ->
+              Forall (fun v => ~ occurs_free e v) (all_fun_name fds) ->
               rw (Efun fds e) e 
 | Fun_rem: forall f t xs fb B1 B2 e,
-             unique_bindings_fundefs (fundefs_append B1 (Fcons f t xs fb B2)) ->
-               num_occur (Efun (fundefs_append B1 (Fcons f t xs fb B2)) e) f 0 -> 
+             unique_name_fundefs (fundefs_append B1 (Fcons f t xs fb B2)) ->
+               num_occur (Efun (fundefs_append B1 (Fcons f t xs fb B2)) e) f 0 ->  
                rw (Efun (fundefs_append B1 (Fcons f t xs fb B2)) e) (Efun (fundefs_append B1 B2) e)
 
 (* Rules about inlining/constant-folding *)
 | Constr_case: forall x c cl co e ys,
-      findtag cl co = Some e ->
-      ~bound_var_ctx c x ->
+    findtag cl co = Some e ->
+    (* x isn't rebind on the way to the case statement *)
+      ~bound_stem_ctx c x ->
       rw (Econstr x co ys (c |[ Ecase x cl ]|)) (Econstr x co ys (c |[e]|))
 
 | Constr_proj: forall v  t t' n x e k ys c, 
                  (* nothing shadows constructor x or var k in c *)
-                 ~ bound_var_ctx c x ->
-                 ~ bound_var_ctx c k ->
-                 (* nothing rebinds the projection k or v in the rest of the term c' *) 
-                 ~ bound_var e v ->
+                 ~ bound_stem_ctx c x ->
+                 ~ bound_stem_ctx c k ->
+                 (* nothing rebinds k in e *)
                  ~ bound_var e k ->
                  x <> k ->
                  v <> k ->
-                 (* everything up could be reduced to ub & Disjoint like in Fun_Inline *) 
                  nthN ys n = Some k -> 
                  rw (Econstr x t ys (c |[Eproj v t' n x e]|)) (Econstr x t ys (c |[ rename k v e]|))
 | Fun_inline: forall c  vs f  t xs fb  fds,
-                (*  nothing rebinds vs's in c'e *)
-                (* could weaken UB assumption *)
-                unique_bindings (Efun fds (c |[ Eapp f t vs ]|))  ->
-                Disjoint var (occurs_free (Efun fds (c |[ Eapp f t vs ]|))) (bound_var (Efun fds (c |[ Eapp f t vs ]|))) ->
-                find_def f fds = Some (t, xs, fb) ->
+    find_def f fds = Some (t, xs, fb) ->
+                (* nothing rebinds vs in \xs.fb *)
+                Disjoint _ (Union _ (FromList xs) (bound_var fb)) (FromList vs) ->
+                unique_name_fundefs fds ->
+                (* nothing shadows the names and FV of fds in c *)
+                Disjoint var (bound_stem_ctx c) (occurs_free_fundefs fds)  ->
+                Disjoint var (bound_stem_ctx c) (name_in_fundefs fds)  -> 
+                List.NoDup xs ->
                 rw (Efun fds (c |[ Eapp f t vs ]|)) (Efun fds (c |[ (rename_all (set_list (combine xs vs) (M.empty var)) fb)]|))                     
 .
          
@@ -286,7 +291,7 @@ Proof.
   specialize (H3 x).
   intro. apply H3; auto.
 Qed.  
-  
+
 
   
 
@@ -326,14 +331,13 @@ Qed.
 
   Corollary  rm_constr :
    forall k rho rho' e' v t l,
-     num_occur e' v 0 ->
+     ~occurs_free e' v ->
   preord_env_P pr cenv (occurs_free (Econstr v t l e')) k rho rho' ->
   preord_exp  pr cenv k (Econstr v t l e', rho) (e', rho').
   Proof.
     intros; intro; intros.
     inversion H2; subst.
     rewrite occurs_free_Econstr in H0.
-    apply not_occurs_not_free in H.
     assert (preord_env_P pr cenv
                          (occurs_free e') k rho rho').
     eapply preord_env_P_antimon.
@@ -346,14 +350,13 @@ Qed.
 
   Corollary rm_prim:
     forall k rho rho' e x p l,
-      num_occur e x 0 ->
+      ~occurs_free e x ->
       preord_env_P pr cenv (occurs_free (Eprim x p l e)) k rho rho' ->
       preord_exp pr cenv k (Eprim x p l e, rho) (e, rho').
   Proof.
         intros; intro; intros.
     inversion H2; subst.
     rewrite occurs_free_Eprim in H0.
-    apply not_occurs_not_free in H.
     assert (preord_env_P pr cenv
                          (occurs_free e) k rho rho').
     eapply preord_env_P_antimon.
@@ -367,14 +370,13 @@ Qed.
 
   Corollary rm_proj:
     forall k rho rho' e x t n y,
-      num_occur e x 0 ->
+      ~occurs_free e x ->
       preord_env_P pr cenv (occurs_free (Eproj x t n y e)) k rho rho' ->
       preord_exp pr cenv k (Eproj x t n y e, rho) (e, rho').
   Proof.
             intros; intro; intros.
     inversion H2; subst.
     rewrite occurs_free_Eproj in H0.
-    apply not_occurs_not_free in H.
     assert (preord_env_P pr cenv
                          (occurs_free e) k rho rho').
     eapply preord_env_P_antimon.
@@ -483,6 +485,21 @@ Qed.
   Qed.
 
 
+    Theorem disjoint_occurs_free_fun: forall e fds,
+  Forall (fun v => ~occurs_free e v) (all_fun_name fds) ->
+  Disjoint var (occurs_free e) (name_in_fundefs fds).
+  Proof.
+    intros.
+    apply Disjoint_intro; intros.
+    intro.
+    inversion H0; subst.
+    rewrite Forall_forall in H.
+    specialize (H x).
+    apply H. 
+    apply all_name_fundefs; auto. auto.
+  Qed.
+
+
   Theorem in_fun_name_suffix: forall fds fds' x,
     List.In x (all_fun_name fds) ->
             fundefs_suffix fds fds' ->
@@ -551,18 +568,44 @@ Qed.
    Qed.
 
    
+   Lemma rm_fundefs_env_of: forall fds' fds e  k rho,
+    Forall (fun v => ~occurs_free e v) (all_fun_name fds') ->
+    fundefs_suffix fds fds' ->
+    preord_env_P pr cenv (occurs_free e) k (def_funs fds' fds rho rho) rho. 
+   Proof.
+     intros.
+     eapply preord_env_P_def_funs_not_in_P_l.
+     apply preord_env_P_refl.
+     apply disjoint_occurs_free_fun.
+     eapply forall_all_fun_name_suffix in H; eauto.
+   Qed.
+
+   Lemma rm_fundefs_env_of': forall fds' fds e  k rho,
+    Forall (fun v => ~occurs_free e v) (all_fun_name fds') ->
+    fundefs_suffix fds fds' ->
+    preord_env_P pr cenv (occurs_free e) k rho (def_funs fds' fds rho rho).  
+   Proof.
+     induction fds; intros.
+     - assert (fundefs_suffix fds fds').
+       unfold fundefs_suffix in *. destruct H0.
+       exists (fundefs_append x (Fcons v f l e Fnil)).
+       rewrite <- H0.
+       rewrite <- fundefs_append_assoc.
+       simpl. reflexivity.       
+       specialize (IHfds _ k rho H H1). 
+       simpl.
+       apply preord_env_P_set_not_in_P_r.
+       auto.
+       split; intro; intro.
+       inv H2. inv H4; subst. revert H3.
+       rewrite Forall_forall in H.
+       apply H.
+       eapply fundefs_suffix_in. 
+       eauto.
+     -simpl. apply preord_env_P_refl.
+   Qed.
 
 
-
-
-     Inductive unique_name_fundefs: fundefs -> Prop :=
-     | Uname_Fcons: forall f tau ys e defs,
-                      ~ name_in_fundefs defs f ->
-                      unique_name_fundefs defs ->
-                      unique_name_fundefs (Fcons f tau ys e defs)
-     | Uname_Fnil:
-         unique_name_fundefs Fnil
-     .
 
 
      Theorem unique_bind_has_unique_name: forall fds,
@@ -585,11 +628,12 @@ Qed.
 
 
        
-     Theorem unique_binding_split: forall fds,
+     Theorem split_fds_unique_name_l: forall fds,
                                      unique_name_fundefs fds ->
                                      forall fds' fds'',
                                        split_fds fds' fds'' fds ->
-                                       unique_name_fundefs fds' /\ unique_name_fundefs fds''.
+                                       unique_name_fundefs fds' /\ unique_name_fundefs fds'' /\
+     Disjoint var (name_in_fundefs fds') (name_in_fundefs fds'').
      Proof.
        induction fds; intros.
        - inversion H; subst.
@@ -601,10 +645,18 @@ Qed.
            constructor.
            intro; apply H3.
            eapply split_fds_name_in_fundefs; eauto.
-           auto. auto.
+           auto.  destruct H2. split; auto. simpl.
+           apply Union_Disjoint_l.
+           apply split_fds_name_in_fundefs in H5.
+           split; intro. intro. apply H3.
+           inv H6. inv H8.
+           apply H5. auto.
+           auto.
          + specialize (IHfds _ _ H5).
            destruct IHfds.
+           destruct H2.
            split.  auto.
+           split. 
            constructor.
            intro.
            apply H3.
@@ -612,10 +664,151 @@ Qed.
            eauto.
            right; auto.
            auto.
+           simpl.
+           apply Union_Disjoint_r.
+           split; intro. intro. apply H3. inv H6.
+           inv H9. eapply split_fds_name_in_fundefs.
+           apply H5. auto.
+           auto.
        - apply split_fds_to_nil in H0.
          destruct H0; subst.
          split; constructor.
+         auto. simpl. auto with Ensembles_DB.
      Qed.
+
+     Lemma split_fds_unique_name_fundefs_r B1 B2 B3 :
+       unique_name_fundefs B1 -> unique_name_fundefs B2 ->
+       Disjoint var (name_in_fundefs B1) (name_in_fundefs B2) ->
+       split_fds B1 B2 B3 ->
+       unique_name_fundefs B3.
+     Proof with eauto with Ensembles_DB.
+       intros Hun1 Hun2 HD Hspl. induction Hspl; simpl; repeat normalize_bound_var_in_ctx.
+       - inv Hun1. constructor; eauto.                  
+         + intros Hc.
+           eapply split_fds_name_in_fundefs in Hc; [| eauto].
+           inv Hc; auto.
+           inv HD. specialize (H0 v). apply H0; split; auto.
+           constructor. auto.
+         + eapply IHHspl...
+       - inv Hun2. constructor; eauto.
+         + intros Hc.
+           eapply split_fds_name_in_fundefs in Hc; [| eauto].
+           inv Hc; auto.
+           inv HD. specialize (H0 v). apply H0; split; auto.
+           constructor. auto.
+         + eapply IHHspl...
+       - constructor.
+     Qed.
+
+     
+     
+     Lemma fundefs_append_unique_name_l B1 B2 B3 :
+       unique_name_fundefs B3 ->
+       fundefs_append B1 B2 = B3 ->
+       unique_name_fundefs B1 /\
+       unique_name_fundefs B2 /\
+       Disjoint var (name_in_fundefs B1) (name_in_fundefs B2).
+     Proof.
+       intros. edestruct split_fds_unique_name_l; eauto.
+       apply fundefs_append_split_fds; eauto.       
+     Qed.
+
+
+     Lemma fundefs_append_unique_name_r B1 B2 B3 :
+       fundefs_append B1 B2 = B3 ->
+       unique_name_fundefs B1 ->
+       unique_name_fundefs B2  ->
+       Disjoint var (name_in_fundefs B1) (name_in_fundefs B2) ->
+       unique_name_fundefs B3.
+     Proof.
+       intros.
+       eapply split_fds_unique_name_fundefs_r;
+         [ apply H0 | | | ]; eauto.
+       apply fundefs_append_split_fds; eauto.
+     Qed.
+
+     
+
+     Theorem fundefs_swap_fun_order2: 
+       forall k x y tx ty xs ys ex ey rho1  B B12 B11',
+         x <> y -> 
+         preord_env pr cenv k (def_funs B (fundefs_append B11' (Fcons x tx xs ex (Fcons y ty ys ey  B12))) rho1 rho1)
+                              (def_funs B (fundefs_append B11' (Fcons y ty ys ey (Fcons  x tx xs ex B12))) rho1 rho1).
+     Proof.
+       induction B11'; intros.
+       - simpl.
+         apply preord_env_extend; auto.
+         apply preord_val_refl.
+       - simpl.
+         intro. intro. intro. intro.
+         rewrite set_permut in H1; auto. exists v1. split; auto.
+         apply preord_val_refl.
+     Qed.         
+
+
+   Theorem  find_def_fundefs_append_none:
+  forall (f : var) (B1 B2 : fundefs) (v : fTag * list var * exp),
+    find_def f B1 = None -> find_def f (fundefs_append B1 B2) = find_def f B2.
+   Proof.
+     induction B1; intros.
+     simpl in *.
+     destruct (M.elt_eq f v); eauto. inv H.
+     simpl. auto.
+   Qed.     
+
+
+
+
+   
+(*
+     Theorem fundefs_swap_val:
+       forall k x y tx ty xs ys ex ey rho1  B12 B11' v,
+         x <> y ->
+         preord_val pr cenv k (Vfun rho1 (fundefs_append B11' (Fcons x tx xs ex (Fcons y ty ys ey B12))) v)
+    (Vfun rho1 (fundefs_append B11' (Fcons y ty ys ey (Fcons x tx xs ex B12))) v).
+     Proof.
+       intros.
+       apply preord_val_eq. intro. intros.
+       assert ( find_def v (fundefs_append B11' (Fcons x tx xs ex (Fcons y ty ys ey B12))) =
+                 find_def v (fundefs_append B11' (Fcons y ty ys ey (Fcons x tx xs ex B12)))).
+       { destruct (find_def v B11') eqn:fd.
+         erewrite find_def_fundefs_append_l; eauto.
+         symmetry.
+         erewrite find_def_fundefs_append_l; eauto.
+         rewrite find_def_fundefs_append_none; auto.
+         rewrite find_def_fundefs_append_none; auto.
+         simpl. destruct (M.elt_eq v x); destruct (M.elt_eq v y); eauto.
+         subst. exfalso. auto.
+       }
+       rewrite H3 in H1. exists xs1, e1.
+       Admitted.
+  *)       
+
+     Theorem rm_fundefs_of': forall k rho e fds,
+    Forall (fun v => ~occurs_free e v) (all_fun_name fds) ->
+    preord_exp pr cenv k (Efun fds e, rho) (e, rho). 
+  Proof.
+    intros; intro; intros.
+    inversion H1; subst.
+    eapply preord_exp_refl in H7; eauto.
+    eapply rm_fundefs_env_of.
+    apply H. exists Fnil. simpl. auto.
+  Qed.
+
+
+  Theorem rm_fundefs_of: forall k rho rho' e fds,
+    Forall (fun v => ~occurs_free e v) (all_fun_name fds) ->
+    preord_env_P pr cenv (occurs_free (Efun fds e))  k rho rho' ->                     
+    preord_exp pr cenv k (Efun fds e, rho) (e, rho'). 
+  Proof.
+    intros.    
+    eapply preord_exp_trans_pre.
+    Focus 2.
+    apply preord_exp_refl.
+    apply H0.
+    intros. eapply preord_val_trans; eauto.
+    intros. apply rm_fundefs_of'. auto.
+  Qed.
 
 
   Theorem rm_fundefs': forall k rho e fds,
@@ -623,10 +816,10 @@ Qed.
     preord_exp pr cenv k (Efun fds e, rho) (e, rho). 
   Proof.
     intros; intro; intros.
-    inversion H1; subst.
-    eapply preord_exp_refl in H7; eauto.
-    eapply rm_fundefs_env.
-    apply H. exists Fnil. simpl. auto.
+    eapply Forall_impl in H.
+    eapply rm_fundefs_of'; eauto.
+    intros.
+    simpl. apply not_occurs_not_free; auto.
   Qed.
 
 
@@ -644,12 +837,13 @@ Qed.
     intros. apply rm_fundefs'. auto.
   Qed.
 
+  
 
 
 
 
   Theorem preord_env_dead_fun: forall f t xs fb k fds' e rho1,
-         num_occur (Efun fds' e) f 0 ->
+           ~(occurs_free (Efun fds' e)) f->
          ~ name_in_fundefs fds' f ->                  
          preord_env_P pr cenv (Union _ (occurs_free (Efun fds' e)) (name_in_fundefs fds')) k (def_funs (Fcons f t xs fb fds') (Fcons f t xs fb fds') rho1 rho1) (def_funs fds' fds' rho1 rho1).
   Proof.
@@ -658,11 +852,7 @@ Qed.
     assert (Hxf: x <> f).
     {
       intro; subst.
-      inv H1.
-      revert H2.
-      apply (proj1 (not_occurs_not_free f)).
-      auto.
-      apply H0. auto.
+      inv H1; auto.
     }
     intro. intros. rewrite M.gso in H2; auto.
     apply Union_Setminus in H1.
@@ -701,7 +891,315 @@ Qed.
     - apply Decidable_name_in_fundefs.
   Qed.
 
+  Theorem find_def_append_not_cons:
+    forall B2 f t xs fb x B1, 
+    x <> f ->
+    find_def x (fundefs_append B1 (Fcons f t xs fb B2)) = find_def x (fundefs_append B1 B2). 
+  Proof.
+    induction B1; intros.
+    - simpl. destruct (M.elt_eq x v); auto.
+    - simpl. destruct (M.elt_eq x f).
+      exfalso; auto.
+      auto.
+  Qed.
+
+  (* adapted from identifiers.fun_in_fundefs_unique_fundefs_split *)
+Lemma fun_in_fundefs_unique_name_split f tau xs e B :
+  fun_in_fundefs B (f, tau, xs, e) ->
+  unique_name_fundefs B ->
+  exists B1 B2,
+    B = fundefs_append B1 (Fcons f tau xs e B2) /\
+    ~ name_in_fundefs B1 f /\
+    Same_set _ (Union _ (fun_in_fundefs B1) (fun_in_fundefs B2))
+             (Setminus _ (fun_in_fundefs B) (Singleton _ (f, tau, xs, e))) /\
+    unique_name_fundefs (fundefs_append B1 B2).
+Proof with eauto with Ensembles_DB.
+  intros H Hun. induction B.
+  - simpl in H.
+    destruct (var_dec v f); subst.
+    + inv H. inv H0.
+      * exists Fnil. eexists. split; simpl; eauto.
+        split; try (now intros Hc; inv Hc). split; try (now inv Hun; eauto).
+        rewrite Union_Empty_set_neut_l, Setminus_Union_distr,
+        Setminus_Same_set_Empty_set, Union_Empty_set_neut_l.
+        symmetry. eapply Setminus_Disjoint.
+        apply Disjoint_Singleton_r. intros Hc.
+        apply fun_in_fundefs_name_in_fundefs in Hc.
+        inv Hun; auto.
+      * exfalso. inv Hun. apply H2. eapply fun_in_fundefs_name_in_fundefs. eauto. 
+    + inv H. inv H0. congruence. inv Hun; eauto.
+      edestruct IHB as [B1 [B2 [Heq [Hn [Hs Hun']]]]]; eauto.
+      edestruct fundefs_append_unique_name_l as [H1 [H2s H3]];
+        [ apply Hun' | | ]; eauto.
+      exists (Fcons v f0 l e0 B1), B2. rewrite Heq. split; eauto.
+      split; [| split ].
+      * intros H. apply Hn. inv H; eauto. inv H4. congruence.
+      * simpl. rewrite Setminus_Union_distr, <- Union_assoc.
+        apply Same_set_Union_compat.
+        apply Same_set_sym. eapply Setminus_Disjoint.
+        apply Disjoint_Singleton_r. intros Hc. inv Hc. congruence.
+        apply Same_set_sym. 
+        rewrite fundefs_append_fun_in_fundefs; eauto. simpl.
+        rewrite !Setminus_Union_distr, Setminus_Same_set_Empty_set,
+        Union_Empty_set_neut_l, <- Setminus_Union_distr.
+        eapply Setminus_Disjoint. apply Union_Disjoint_l.
+        eapply Disjoint_Singleton_r. intros Hc. 
+        apply Hn.
+        eapply fun_in_fundefs_name_in_fundefs; eauto.
+        eapply Disjoint_Singleton_r. intro.
+        assert (In _ (Union (var * fTag * list var * exp) (fun_in_fundefs B1) (fun_in_fundefs B2)) (f, tau, xs, e)). right; auto. rewrite Hs in H4. inv H4. apply H7. auto.
+      * simpl. constructor; eauto.
+        intros H. apply H2.
+        eapply fundefs_append_name_in_fundefs.
+        symmetry. apply Heq.
+        eapply fundefs_append_name_in_fundefs in H; [|reflexivity].
+        inv H; auto.
+        right. constructor 2. auto.
+  - inv H.
+Qed.
+
+Lemma find_def_Included_name_in_fundefs f B B' :
+  unique_name_fundefs B ->
+  unique_name_fundefs B' ->
+  Included _ (fun_in_fundefs B) (fun_in_fundefs B') ->
+  name_in_fundefs B f ->
+  find_def f B = find_def f B'.
+Proof with eauto with Ensembles_DB.
+  revert B'. induction B; simpl; intros B' Hun Hun' H Hn.
+  - edestruct fun_in_fundefs_unique_name_split
+      as [B1 [B1' [Heq [Hn' [HS' Hun1]]]]]; eauto.
+    eapply H. left. eauto.
+    rewrite Heq. destruct (M.elt_eq f v); subst.
+    + erewrite find_def_fundefs_append_r.
+      simpl; destruct (M.elt_eq v v); try congruence.
+      simpl; destruct (M.elt_eq v v); try congruence. eauto.
+      apply name_not_in_fundefs_find_def_None.
+      intros Hc. apply Hn'; eauto.
+    + rewrite find_def_fundefs_append_Fcons_neq; eauto. eapply IHB; eauto.
+      inv Hun; eauto.
+      rewrite (fundefs_append_fun_in_fundefs B1 B1' (fundefs_append B1 B1')); eauto.
+      eapply Included_trans; [| inv HS'; eauto].
+      rewrite <- (Setminus_Disjoint (fun_in_fundefs B) (Singleton _ (v, f0, l, e))).
+      eapply Included_Setminus_compat...
+      eapply Included_trans; [| eassumption ]...
+      eapply Disjoint_Singleton_r. inv Hun; eauto. intros Hc. apply H2.
+      now eapply fun_in_fundefs_name_in_fundefs; eauto.
+      inv Hn. inv H0; try congruence. eauto.
+  - destruct B'; eauto. inv Hn.
+Qed.
+
+
+Lemma find_def_Same_set_name_in_fundefs f B B' :
+  unique_name_fundefs B ->
+  unique_name_fundefs B' ->
+  Same_set _ (fun_in_fundefs B) (fun_in_fundefs B') ->
+  find_def f B = find_def f B'.
+Proof.
+  intros Hun1 Hun2 HS.
+  destruct (@Dec _ _ (Decidable_name_in_fundefs B) f).
+  - inv HS. eapply find_def_Included_name_in_fundefs; eauto.
+  - rewrite !name_not_in_fundefs_find_def_None; eauto.
+    intros Hn. apply H.
+    apply name_in_fundefs_big_cup_fun_in_fundefs in Hn.
+    destruct Hn as [[[[f' t] xs] e] [H1 H2]]. inv H2.
+    eapply fun_in_fundefs_name_in_fundefs. now eapply HS; eauto.
+Qed.
+
+(* stronger version of preord_env_P_Same_set_fun_in_fundefs *)
+    Lemma preord_env_P_Same_set_name_in_fundefs k S1 B1 B1' B2 B2' rho1 rho1' :
+    Same_set _ (fun_in_fundefs B1) (fun_in_fundefs B2) ->
+    Same_set _ (fun_in_fundefs B1') (fun_in_fundefs B2') ->
+    unique_name_fundefs B1'->
+    unique_name_fundefs B1 ->
+    unique_name_fundefs B2'->
+    unique_name_fundefs B2 ->
+    preord_env_P pr cenv S1 k (def_funs B1' B1 rho1 rho1') (def_funs B2' B2 rho1 rho1').
+  Proof. 
+    revert B1 S1 B1' B2 B2' rho1 rho1'. induction k using lt_wf_rec1.
+    induction B1; intros S1 B1' B2 B2' rho1 rho1' HS1 HS2 Hun1' Hun1 Hun2' Hun2.    
+    - edestruct fun_in_fundefs_unique_name_split
+      with (B := B2) as [B [B' [Heq [Hn [HS Hun']]]]]; eauto.
+      eapply HS1. left. eauto.
+      edestruct fundefs_append_unique_name_l as [H1 [H2 H3]]; eauto.
+      rewrite Heq. 
+      eapply preord_env_P_antimon;
+        [| apply (@Included_Union_Setminus _ _ (Singleton var v) _)].
+      eapply preord_env_P_union.
+      + simpl. eapply preord_env_P_set_not_in_P_l;
+          eauto using Disjoint_Setminus_l, Included_refl.
+        eapply preord_env_P_trans;
+          [| intros m; apply proerd_env_P_def_funs_weakening; intros Hc; inv Hc; eauto ].
+        eapply IHB1; eauto ; try (now inv Hun1; eauto).
+        rewrite (fundefs_append_fun_in_fundefs B B' (fundefs_append B B')); eauto.
+        rewrite HS, <- HS1. eauto with Ensembles_DB. simpl.
+        rewrite Setminus_Union_distr, Setminus_Same_set_Empty_set, Union_Empty_set_neut_l.
+        inv Hun1. rewrite Setminus_Disjoint; eauto with Ensembles_DB.
+        eapply Disjoint_Singleton_r.
+        intros Hc. apply H5.
+        eapply fun_in_fundefs_name_in_fundefs; eauto.
+      + rewrite def_funs_append;
+        eapply preord_env_P_def_funs_not_in_P_r.
+        * simpl. eapply preord_env_P_extend.
+          rewrite Setminus_Same_set_Empty_set. apply preord_env_Empty_set.
+          rewrite preord_val_eq. intros vs1 vs2 j t1 xs1 e1 rho1'' Hlen Hf Hs. 
+          edestruct (@setlist_length val) as [rho2'' Hs']; [eauto | | ]. eauto.
+          exists xs1, e1, rho2''. repeat split; eauto.
+          erewrite <- find_def_Same_set_name_in_fundefs; eauto.
+          intros Hleq Hpre'. eapply preord_exp_refl; eauto.
+          eapply preord_env_P_setlist_l; [| | | eauto | eauto ]; eauto.
+        * eauto with Ensembles_DB.
+    - simpl. destruct B2; eauto using preord_env_P_refl.
+      destruct HS1 as [_ H1]. exfalso. eapply not_In_Empty_set. eapply H1.
+      simpl. eauto.
+  Qed.
+
+
+
+  (*
+  Theorem preord_env_dead_fun_of: forall f t xs fb   B1' k B1 B2 e rho1,
+      ~occurs_free (Efun (fundefs_append B1 B2) e) f->
+      ~ name_in_fundefs (fundefs_append B1 B2) f ->
+      fundefs_suffix B1' B1 ->
+      preord_env_P pr cenv (Union _ (occurs_free (Efun (fundefs_append B1 B2) e)) (name_in_fundefs (fundefs_append B1 B2))) k (def_funs (fundefs_append B1 (Fcons f t xs fb B2)) (fundefs_append B1' (Fcons f t xs fb B2)) rho1 rho1) (def_funs (fundefs_append B1 B2) (fundefs_append B1' B2) rho1 rho1).
+      Proof.
+      induction B1'; intros.
+      - simpl.
+        eapply preord_env_P_extend.
+        eapply preord_env_P_antimon.
+        apply IHB1'; eauto.
+        inv H1.
+        exists (fundefs_append x (Fcons v f0 l e Fnil)).
+        rewrite <- fundefs_append_assoc. simpl. auto.
+        eauto with Ensembles_DB.
+        
+        admit.
+        
+      - simpl. eapply preord_env_P_set_not_in_P_l; eauto.
+        Focus 2. eauto with Ensembles_DB.
+         admit.
+  Admitted.
+*)
+        (*
   
+    Lemma preord_env_dead_rm_fun_df: forall f t xs fb  k B1 B2 e B rho1 rho2,
+         ~occurs_free (Efun (fundefs_append B1 B2) e) f->
+         ~ name_in_fundefs (fundefs_append B1 B2) f ->
+         ~ name_in_fundefs B f ->
+         preord_env_P pr cenv (Union _ (occurs_free (Efun (fundefs_append B1 B2) e)) (name_in_fundefs (fundefs_append B1 B2))) k rho1 rho2 ->
+         preord_env_P pr cenv (Union _ (occurs_free (Efun (fundefs_append B1 B2) e)) (name_in_fundefs (fundefs_append B1 B2))) k (def_funs (fundefs_append B1 (Fcons f t xs fb B2)) B rho1 rho1) (def_funs (fundefs_append B1 B2) B rho2 rho2).
+    Proof.
+      induction B; intros.      
+      - simpl.  apply preord_env_P_extend.
+        + eapply preord_env_P_antimon.
+          apply IHB; eauto. intro; apply H1. constructor 2. auto.
+          eauto with Ensembles_DB.
+        + apply preord_val_eq.
+          intro; intros.           
+          exists xs1, e1.
+          rewrite find_def_append_not_cons in H4.
+          assert (exists rho2', 
+    setlist xs1 vs2
+            (def_funs (fundefs_append B1 B2) (fundefs_append B1 B2) rho2 rho2) = Some rho2').
+          eapply setlist_length. Focus 2. symmetry. apply H5. auto.
+          destruct H6. exists x. split; auto. split; auto. intros.
+          Focus 2. intro; apply H1. constructor. subst. constructor.
+          apply preord_exp_refl.
+          eapply preord_env_P_setlist_l; eauto.
+          
+          admit.
+      - simpl. apply H2.
+Admitted.      *)
+
+      (*
+    Theorem preord_env_dead_fun_of: forall f t xs fb  B1 B2 e B1' k rho1,
+         ~occurs_free (Efun (fundefs_append B1 B2) e) f->
+         ~ name_in_fundefs (fundefs_append B1 B2) f ->
+         fundefs_suffix B1' B1 ->
+         preord_env_P pr cenv (Union _ (occurs_free (Efun (fundefs_append B1 B2) e)) (name_in_fundefs (fundefs_append B1 B2))) k (def_funs (fundefs_append B1 (Fcons f t xs fb B2)) (fundefs_append B1' (Fcons f t xs fb B2)) rho1 rho1) (def_funs (fundefs_append B1 B2) (fundefs_append B1' B2) rho1 rho1).
+    Proof.
+      intros. 
+      do 2 (rewrite def_funs_append).   simpl. SearchAbout def_funs. 
+       induction B1'. 
+      - simpl.
+
+        intros; intro; intros.
+        assert (Hxf: x <> f).
+        {
+          intro; subst.
+          inv H2.
+          auto.
+          auto.
+        }
+        simpl.
+        apply preord_var_env_extend.
+        apply IHB1'. inv H1.
+        exists (fundefs_append x0 (Fcons v f0 l e0 Fnil)).
+        rewrite <- fundefs_append_assoc. simpl. auto.
+        auto.
+        apply preord_val_eq.
+          intro; intros.           
+          exists xs1, e1.
+          rewrite find_def_append_not_cons in H4.
+          assert (exists rho2', 
+                    setlist xs1 vs2
+            (def_funs (fundefs_append B1 B2) (fundefs_append B1 B2) rho1 rho1) = Some rho2').
+          eapply setlist_length. Focus 2. symmetry. apply H5. auto.
+          destruct H6. exists x0. split; auto. split; auto. intros.
+          Focus 2. intro; subst. apply H0.
+          inv H1.
+          eapply fundefs_append_name_in_fundefs. reflexivity.
+          left.
+          eapply fundefs_append_name_in_fundefs.  reflexivity. right. constructor. auto.
+          eapply preord_exp_refl. SearchAbout preord_env_P setlist.
+          eapply preord_env_P_setlist_l; eauto.
+          
+      - intros.
+        simpl.
+        apply preord_env_P_set_not_in_P_l.
+        
+        admit.
+        eauto with Ensembles_DB.
+      
+    
+    
+    intro. intros. rewrite M.gso in H2; auto.
+    apply Union_Setminus in H1.
+    inv H1.
+    - inv H3.  rewrite def_funs_neq; auto.
+      rewrite def_funs_neq in H2; auto.
+      exists v1; split; auto.
+      apply preord_val_refl.
+    - erewrite def_funs_eq in H2; auto.
+      inv H2.
+      erewrite def_funs_eq; auto.
+      exists  (Vfun rho1 fds' x).
+      split; auto.
+      rewrite preord_val_eq. intro. intros.
+      assert (fundefs_append Fnil (Fcons f t xs fb fds') = (Fcons f t xs fb fds')) by auto.
+      rewrite <- H5 in H2.
+      rewrite find_def_fundefs_append_Fcons_neq in H2; auto. simpl in H2. 
+      clear H5.
+      symmetry in H4.
+      assert (Hsl:= setlist_length _ (def_funs fds' fds' rho1 rho1) _ _ _  _ H1 H4).
+      destruct Hsl.
+      exists xs1, e1, x0.
+      split; auto. split; auto.
+      intros.
+      eapply preord_exp_refl.      
+      eapply preord_env_P_setlist_l; eauto.  intros.
+      apply find_def_correct in H2.
+      eapply occurs_free_in_fun in H9; eauto.
+      inv H9.
+      exfalso; apply H8; auto.
+      inv H10.
+      right; auto.
+      left.
+      rewrite occurs_free_Efun. left.
+      auto.
+    - apply Decidable_name_in_fundefs.
+  Qed.
+
+  *)
 
 
   Theorem rm1_fundefs: forall k rho1 rho2 fb e fds xs t f ,
@@ -720,11 +1218,12 @@ Qed.
       eapply preord_exp_refl in H7. Focus 2.
       eapply preord_env_P_antimon.
       apply preord_env_dead_fun with (e := e). 
-      inv H; subst. apply plus_is_O in H3. destruct H3; subst. constructor; auto.
-      inv H6. apply plus_is_O in H10. destruct H10; subst. simpl; auto.
+      inv H; subst. apply plus_is_O in H3. destruct H3; subst.
+      apply not_occurs_not_free. rewrite <- plus_0_r.
+      constructor. auto. inv H6; pi0; auto.
       auto.
       rewrite occurs_free_Efun.
-      intro. intros.
+      intro. intro.
       assert (Hv := Decidable_name_in_fundefs fds).
       inv Hv. specialize (Dec x).
       destruct Dec. right; auto.
@@ -735,7 +1234,6 @@ Qed.
       constructor. auto.
       auto.
   Qed.
-
 
 
       Lemma split_fds_unique_bindings_lr:
@@ -784,9 +1282,9 @@ Qed.
           constructor; auto. split; auto. omega.
         -         simpl in H. exists 0, nm. split; auto. constructor.
       Qed.
-      
+
   Theorem rm_any_fundefs: forall k rho1 rho2 fb e B1 B2 B xs t f ,
-                            unique_bindings_fundefs B ->
+                            unique_name_fundefs B ->
                             fundefs_append B1 (Fcons f t xs fb B2) = B ->
                             num_occur (Efun B e) f 0 -> 
                          preord_env_P pr cenv (occurs_free (Efun B e)) k rho1 rho2 -> 
@@ -800,33 +1298,18 @@ Qed.
          Focus 2. reflexivity. symmetry. rewrite fundefs_append_fun_in_fundefs.
          Focus 2. reflexivity. simpl. eauto with Ensembles_DB.
     }
-    assert (Hub : unique_bindings_fundefs (fundefs_append (Fcons f t xs fb B1) B2)). {
-      eapply fundefs_append_unique_bindings_l in H. 2: reflexivity.
+    assert (Hub : unique_name_fundefs (fundefs_append (Fcons f t xs fb B1) B2)). {
+      eapply fundefs_append_unique_name_l in H. 2: reflexivity.
       destructAll. inv H3. simpl. constructor; auto.
-      rewrite bound_var_fundefs_Fcons in H4.
-      intro.
-      eapply fundefs_append_bound_vars in H3.
-      2: reflexivity.
-      inv H4. specialize (H5 f). 
-      inv H3.
-      apply H5. eauto with Ensembles_DB.
-      apply H11. auto.
-      rewrite bound_var_fundefs_Fcons in H4.
-      erewrite fundefs_append_bound_vars.
-      2: reflexivity.
-      eauto with Ensembles_DB.
-      rewrite bound_var_fundefs_Fcons in H4.
-      erewrite fundefs_append_bound_vars.
-      2: reflexivity.
-      eauto with Ensembles_DB.
-      eapply fundefs_append_unique_bindings_r.
+      intro. eapply fundefs_append_name_in_fundefs in H3; [| reflexivity]. inv H3; auto.
+      inv H4. specialize (H3 f). apply H3. split; auto.
+      constructor. auto.
+      eapply fundefs_append_unique_name_r.
       reflexivity.
       auto.
       auto.
-      rewrite bound_var_fundefs_Fcons in H4.
       eauto with Ensembles_DB.
-    }
-    
+    }    
     eapply preord_exp_trans.
     apply preord_exp_refl. apply H2.
     intros.
@@ -835,7 +1318,7 @@ Qed.
       inv H4. eapply preord_exp_refl in H10.
       Focus 2.
       
-      eapply preord_env_P_Same_set_fun_in_fundefs.
+      eapply preord_env_P_Same_set_name_in_fundefs.
       apply H0.
       apply H0.
       auto. auto.
@@ -852,16 +1335,16 @@ Qed.
       eapply preord_env_P_antimon.
       apply preord_env_dead_fun with (e := e).
       inv H1. apply plus_is_O in H6. destruct H6; subst.
-      constructor. auto.
       apply fundefs_append_num_occur' in H9. destructAll.
       inv H4. apply plus_is_O in H5. destruct H5.
-      apply plus_is_O in H5. destruct H5; subst. rewrite <- plus_0_l.
+      apply plus_is_O in H5. destruct H5; subst.
+      apply not_occurs_not_free.
+      rewrite <- plus_0_l. constructor; auto.
+      rewrite <-plus_0_l.
       eapply fundefs_append_num_occur. reflexivity.
       auto. auto.
-      inv Hub.
-      intro; apply H11.
-      apply name_in_fundefs_bound_var_fundefs. auto.
-      rewrite occurs_free_Efun.
+      simpl in Hub. inv Hub. auto.
+      rewrite occurs_free_Efun. 
       intro. intros.
       assert (Hv := Decidable_name_in_fundefs (fundefs_append B1 B2)).
       inv Hv. specialize (Dec x).
@@ -872,8 +1355,9 @@ Qed.
       split; eauto.
       constructor. auto.
       auto.
-Qed.      
+Qed.
       
+  
   Theorem proper_getlist: forall A rho rho',
     map_get_r A rho rho' ->
     forall vs, getlist vs rho = getlist vs rho'.
@@ -1078,7 +1562,7 @@ Theorem bv_in_ctx: (forall c e x c',
       apply bound_var_Case_c. right. left. eapply IHe; eauto.
       apply bound_var_Case_c; auto.
     + destruct a. inversion H3; subst.
-      apply bound_var_Case_c in H0.
+      apply bound_var_Case_c in H0. 
       inv H0.
       inversion H1; subst. inversion H6.
       inv H1. apply bound_var_Case_c.
@@ -1193,6 +1677,8 @@ Theorem bv_in_ctx: (forall c e x c',
 Qed.
 
 
+  
+
     
 Theorem bv_in_find_def_ctx2: forall x f t1 e xs1 c B, 
   find_def f (B<[e]>) = Some (t1, xs1, c |[ e ]|) ->
@@ -1208,6 +1694,8 @@ Proof.
         constructor 7. apply bound_var_app_ctx. left. auto.
   - apply IHB in H; auto.
 Qed.
+
+
 
 
 
@@ -1476,16 +1964,6 @@ Qed.
    auto.
  Qed.
 
-Theorem Decidable_singleton_var: forall v, Decidable (Singleton var v).
-Proof.
-  intro.
-  apply Build_Decidable.
-  intro.
-  destruct (var_dec v x).
-  subst; left; constructor.
-  right; intro.
-  apply n; inversion H; auto.
-Qed.
 
  
  Definition eq_env_P {A}:  Ensemble var -> M.t A -> M.t A -> Prop :=
@@ -1689,6 +2167,134 @@ Proof.
 Qed.    
 
 
+
+ 
+
+
+
+(* More precise statement of find_def_def_funs_ctx *)
+  Lemma find_def_def_funs_ctx' B f e1 tau xs e' :
+    find_def f (B <[ e1 ]>) = Some (tau, xs, e') ->
+    (forall e2, (find_def f (B <[ e2 ]>) = Some (tau, xs, e'))) \/
+    (exists c, e' = c |[ e1 ]| /\
+              (forall e2, find_def f (B <[ e2 ]>) = Some (tau, xs, c |[ e2 ]|)) /\ (exists fd fd', B = (app_fundefs_ctx fd (Fcons1_c f tau xs c fd')))).
+  Proof.
+    revert tau xs e'. induction B; simpl; intros tau xs e' Heq.
+    - destruct (M.elt_eq f v).
+      + inv Heq. right. eexists e.
+        split; eauto.
+        split; eauto. exists Fnil, f0; auto.
+      + left; eauto.
+    - destruct (M.elt_eq f v).
+      + inv Heq. left; eauto.
+      + apply IHB in Heq. inv Heq. left; auto.
+        inv H. destruct H0.
+        inv H0. right.  exists x. split; auto. split; auto. destruct H2. destruct H.
+        exists (Fcons v c l e x0), (x1).
+        simpl. rewrite H. auto.        
+  Qed.
+
+  
+
+    
+  Lemma preord_env_P_def_funs_compat_pre_vals_stem_set S k B  rho1 rho2 B' e1 e2 S1 :
+    (forall m c (rho1' rho2' : env),
+       m <  k ->
+       Disjoint var (bound_stem_ctx c) S ->
+       eq_env_P S rho1 rho1' -> 
+       eq_env_P S rho2 rho2' -> 
+       preord_env_P pr cenv (occurs_free (c |[ e1 ]|)) m rho1' rho2' ->
+       preord_exp pr cenv m (c |[ e1 ]|, rho1') (c |[ e2 ]|, rho2')) ->
+    preord_env_P pr cenv (Union _ (occurs_free_fundefs (B' <[ e1 ]>))
+                        (Setminus _ S1 (name_in_fundefs (B' <[ e1 ]>))))
+                 k rho1 rho2 ->
+    Disjoint var (Union var (names_in_fundefs_ctx B) (bound_stem_fundefs_ctx B)) S ->
+    Disjoint var (Union var (names_in_fundefs_ctx B') (bound_stem_fundefs_ctx B')) S ->
+    preord_env_P pr cenv (Union _ (Setminus _ S1 (name_in_fundefs (B' <[ e1 ]>)))
+                        (Union _ (occurs_free_fundefs (B' <[ e1 ]>))
+                               (name_in_fundefs (B <[ e1 ]>))))
+                 k (def_funs (B' <[ e1 ]>) (B <[ e1 ]>) rho1 rho1)
+                 (def_funs (B' <[ e2 ]>) (B <[ e2 ]>) rho2 rho2).
+  Proof.
+    revert B rho1 rho2 B' e1 e2 S1.
+    induction k as [ k IH' ] using lt_wf_rec1.
+    intros B rho1 rho2 B' e1 e2 S1 Hpre Henv Hbv Hbv'.
+    assert (Hval : forall f, preord_val pr cenv k (Vfun rho1 (B' <[ e1 ]>) f)
+                                   (Vfun rho2 (B' <[ e2 ]>) f)).
+    { intros f. rewrite preord_val_eq.
+      intros vs1 vs2 j t1 xs1 e' rho1' Hlen Hf Hs.
+      edestruct find_def_def_funs_ctx' as [H1 | [c [H1 H2]]]; eauto.
+      
+      + edestruct (@setlist_length cps.val) as [rho2' Hs']; eauto.
+        do 4 eexists; eauto. split; eauto.
+        intros Hleq Hall.
+        eapply preord_exp_refl.
+        eapply preord_env_P_setlist_l; [| | now eauto | now eauto | now eauto ].
+        eapply IH'; eauto. 
+        intros. eapply Hpre; eauto. omega. 
+        eapply preord_env_P_monotonic; [| eassumption ]. omega.
+        intros x0 H Hfv. 
+        eapply find_def_correct in Hf; eauto.
+        eapply occurs_free_in_fun in Hfv; eauto.
+        inv Hfv. exfalso. eauto.  right. eapply Ensembles_util.Union_commut. eauto.
+      + destruct H2. inv H0. inv H2. 
+        edestruct (@setlist_length cps.val) as [rho2' Hs']; eauto.
+        do 4 eexists; eauto.
+        split; eauto.
+        intros Hleq Hall. eapply Hpre; eauto.
+        {
+          split; intro; intro. rewrite bound_stem_app_fundefs_ctx in Hbv'.
+          inv Hbv'. specialize (H1 x1). apply H1. inv H0; auto.
+        }
+        eapply eq_env_P_setlist_not_in_P_r; eauto.
+        
+        
+        apply eq_env_P_def_funs_not_in_P_r. apply eq_env_P_refl.
+
+        rewrite <- name_in_fundefs_ctx_ctx.
+        eauto with Ensembles_DB.
+        rewrite bound_stem_app_fundefs_ctx in Hbv'.
+        eauto with Ensembles_DB.
+
+        symmetry in Hs'.
+        intro; eapply eq_env_P_setlist_not_in_P_r; eauto.
+        apply eq_env_P_def_funs_not_in_P_r.
+        apply eq_env_P_refl.
+        rewrite <- name_in_fundefs_ctx_ctx.
+        eauto with Ensembles_DB.
+        rewrite bound_stem_app_fundefs_ctx in Hbv'.
+        eauto with Ensembles_DB.
+
+        eapply preord_env_P_setlist_l; [| | eauto | eauto | eauto ].
+        eapply IH'; eauto.
+        intros. eapply Hpre; eauto. omega. 
+        eapply preord_env_P_monotonic; [| eassumption ]. omega.
+        intros x1 Hv Hfv. 
+        eapply find_def_correct in Hf; eauto.
+        eapply occurs_free_in_fun in Hfv; eauto.
+        inv Hfv. exfalso. eauto. right. eapply Ensembles_util.Union_commut. eauto. }
+    induction B.
+    - simpl. apply preord_env_P_extend.
+      + clear Hbv. induction f.
+        { simpl. apply preord_env_P_extend.
+          - eapply preord_env_P_antimon; [ eassumption |].
+            rewrite Ensembles_util.Setminus_Union.
+            eauto 15 with Ensembles_DB typeclass_instances.
+          - eapply Hval. }
+        { simpl. eapply preord_env_P_antimon ; [ eassumption |].
+          eauto with Ensembles_DB. }
+      + eapply Hval.
+    - simpl. apply preord_env_P_extend.
+      + eapply preord_env_P_antimon. apply IHB.
+        eapply Disjoint_Included_l.        
+        2: apply Hbv.
+        apply Included_Union_compat.
+        simpl. right; auto.
+        rewrite bound_stem_Fcons2_c. reflexivity. 
+        eauto 10 with Ensembles_DB.
+      + apply Hval.
+  Qed.
+ 
 Lemma preord_env_P_def_funs_compat_pre_vals_set S k B  rho1 rho2 B' e1 e2 S1 :
     (forall m c (rho1' rho2' : env),
        m <  k ->
@@ -1737,9 +2343,9 @@ Lemma preord_env_P_def_funs_compat_pre_vals_set S k B  rho1 rho2 B' e1 e2 S1 :
           specialize (H x).
           apply H. split; auto.
           eapply bv_in_find_def_ctx2; eauto.
-        }
+        } 
         eapply eq_env_P_setlist_not_in_P_r; eauto.
-        apply eq_env_P_def_funs_not_in_P_r. apply eq_env_P_refl.
+        apply eq_env_P_def_funs_not_in_P_r. apply eq_env_P_refl. 
         split. intros. intro. destruct H.
         apply name_boundvar_ctx in H0.
         inv Hbv'. specialize (H1 x). auto.
@@ -1786,15 +2392,17 @@ Lemma preord_env_P_def_funs_compat_pre_vals_set S k B  rho1 rho2 B' e1 e2 S1 :
       + apply Hval.
   Qed.
 
-(*This means that only bound variables in the applicative context c will modify the evaluation context rho *)
-    Lemma preord_exp_compat_vals_set S k rho1 rho2 c e1 e2 :
+
+  
+(*This means that only bound variables on the applicative context c will modify the evaluation context rho *)
+    Lemma preord_exp_compat_vals_stem_set S k rho1 rho2 c e1 e2 :
       (forall k' rho1' rho2', k' <= k ->
                               preord_env_P pr cenv (occurs_free e1) k' rho1' rho2' ->
                               
                               eq_env_P S rho1 rho1' ->
                               eq_env_P S rho2 rho2' ->
                               preord_exp pr cenv k' (e1, rho1') (e2, rho2')) ->
-    Disjoint var (bound_var_ctx c) S ->
+    Disjoint var (bound_stem_ctx c) S ->
     preord_env_P pr cenv (occurs_free (c |[ e1 ]|)) k rho1 rho2 ->
     preord_exp pr cenv k (c |[ e1 ]|, rho1) (c |[ e2 ]|, rho2).
   Proof.
@@ -1804,7 +2412,7 @@ Lemma preord_env_P_def_funs_compat_pre_vals_set S k B  rho1 rho2 B' e1 e2 S1 :
       simpl in Hpre. apply Hpre.
       apply eq_env_P_refl.
       apply eq_env_P_refl.
-    -         rewrite bound_var_Econstr_c in Hbv. 
+    -  rewrite bound_stem_Econstr_c in Hbv. simpl.  
       eapply preord_exp_const_compat; eauto; intros.
       * eapply Forall2_same. intros x0 HIn. apply Hpre. constructor. auto.
       * assert (Disjoint _ S (Singleton _ v)).
@@ -1829,7 +2437,7 @@ Lemma preord_env_P_def_funs_compat_pre_vals_set S k B  rho1 rho2 B' e1 e2 S1 :
         rewrite preord_val_eq. constructor. reflexivity.
         apply Forall2_Forall2_asym_included; auto.
     - simpl app_ctx_f.
-      rewrite bound_var_Eproj_c in Hbv.
+      rewrite bound_stem_Eproj_c in Hbv.
       eapply preord_exp_proj_compat; eauto.
       + eapply Hpre. constructor; eauto.
       + intros vs1 vs2 Hall.
@@ -1850,7 +2458,7 @@ Lemma preord_env_P_def_funs_compat_pre_vals_set S k B  rho1 rho2 B' e1 e2 S1 :
         simpl. rewrite occurs_free_Eproj.
         eauto with Ensembles_DB.
     - simpl.
-      rewrite bound_var_Eprim_c in Hbv.
+      rewrite bound_stem_Eprim_c in Hbv.
       eapply preord_exp_prim_compat; eauto.
       + eapply Forall2_same. intros x0 Hin. eapply Hpre. constructor; eauto.
       + intros vs1 vs2 Hall.
@@ -1872,22 +2480,21 @@ Lemma preord_env_P_def_funs_compat_pre_vals_set S k B  rho1 rho2 B' e1 e2 S1 :
         eauto with Ensembles_DB.
     - simpl. eapply preord_exp_case_compat; eauto.
       eapply IHc; auto.      
-      rewrite bound_var_Case_c in Hbv.
+      rewrite bound_stem_Case_c in Hbv.
       eapply Disjoint_Included_l; eauto.
-      right. left; auto.
+      reflexivity.      
       eapply preord_env_P_antimon; eauto.
       simpl. intros x0 H.
       eapply occurs_free_Ecase_Included; eauto.
       eapply in_or_app. right. left; eauto.
     - simpl.
-      rewrite bound_var_Fun1_c in Hbv.
+      rewrite bound_stem_Fun1_c in Hbv.
       eapply preord_exp_fun_compat; eauto.      
       assert (Disjoint _ S (name_in_fundefs f)).
       {
         eapply Disjoint_Included_l in Hbv.
         apply Disjoint_sym. apply Hbv.
         left.
-        apply name_in_fundefs_bound_var_fundefs.
         auto.
         } 
         eapply IHc; eauto.
@@ -1905,16 +2512,16 @@ Lemma preord_env_P_def_funs_compat_pre_vals_set S k B  rho1 rho2 B' e1 e2 S1 :
     - intros v1 c1 Hleq Hstep. inv Hstep.
       edestruct (preord_exp_refl pr cenv k e) as [v2 [c2 [Hstep1 Henv2]]]; eauto.
       + eapply preord_env_P_antimon.
-        * rewrite bound_var_Fun2_c in Hbv.
+        * rewrite bound_stem_Fun2_c in Hbv.
           assert (Hbv' := Disjoint_Union_l  _ _ _ Hbv).
-          eapply preord_env_P_def_funs_compat_pre_vals_set; eauto.
+          eapply preord_env_P_def_funs_compat_pre_vals_stem_set; eauto.
           intros. eapply IH'; eauto.
           intros.
           eapply Hyp; eauto.
           omega.
           eapply eq_env_P_trans.
-          apply H1. auto.
-          eapply eq_env_P_trans. apply H2. auto.
+          apply H1. auto.          
+          eapply eq_env_P_trans; eauto.
           eapply preord_env_P_antimon; [ eassumption |].
           intros x' H'. simpl. inv H'.
           now eapply Free_Efun2.
@@ -1925,6 +2532,26 @@ Lemma preord_env_P_def_funs_compat_pre_vals_set S k B  rho1 rho2 B' e1 e2 S1 :
       + repeat eexists; eauto. simpl. constructor; eauto.
   Qed.
 
+
+  (*This means that only bound variables on the applicative context c will modify the evaluation context rho *)
+    Lemma preord_exp_compat_vals_set S k rho1 rho2 c e1 e2 :
+      (forall k' rho1' rho2', k' <= k ->
+                              preord_env_P pr cenv (occurs_free e1) k' rho1' rho2' ->
+                              
+                              eq_env_P S rho1 rho1' ->
+                              eq_env_P S rho2 rho2' ->
+                              preord_exp pr cenv k' (e1, rho1') (e2, rho2')) ->
+    Disjoint var (bound_var_ctx c) S ->
+    preord_env_P pr cenv (occurs_free (c |[ e1 ]|)) k rho1 rho2 ->
+    preord_exp pr cenv k (c |[ e1 ]|, rho1) (c |[ e2 ]|, rho2).
+  Proof.
+    intros.
+    eapply preord_exp_compat_vals_stem_set; eauto.
+    eapply Disjoint_Included_l; eauto.
+    apply bound_stem_var.
+  Qed.
+
+  
     (* almost generalization of preord_exp_combat_vals_le (and val) to sets-> would need rho1 = rho1' /\ rho2 = rho2' on S *)
      Corollary preord_exp_compat_vals_set' S k rho1 rho2 c e1 e2 :
       (forall k' rho1' rho2', k' <= k ->
@@ -1948,6 +2575,28 @@ Lemma preord_env_P_def_funs_compat_pre_vals_set S k B  rho1 rho2 B' e1 e2 S1 :
   Qed.
 
   
+  Corollary preord_exp_compat_stem_vals_le xs vs vs' k rho1 rho2 c e1 e2 :
+      (forall k' rho1 rho2, preord_env_P pr cenv (occurs_free e1) k' rho1 rho2 ->
+                           k' <= k ->
+                         getlist xs rho1 = Some vs ->
+                         getlist xs rho2 = Some vs' -> 
+                         preord_exp pr cenv k' (e1, rho1) (e2, rho2)) ->
+    Disjoint var (bound_stem_ctx c) (FromList xs) ->
+    getlist xs rho1 = Some vs ->
+    getlist xs rho2 = Some vs' -> 
+    preord_env_P pr cenv (occurs_free (c |[ e1 ]|)) k rho1 rho2 ->
+    preord_exp pr cenv k (c |[ e1 ]|, rho1) (c |[ e2 ]|, rho2).
+  Proof.
+    intros.
+    eapply preord_exp_compat_vals_stem_set with (S := FromList xs); eauto.
+    intros. apply H; eauto.
+    erewrite <- eq_env_P_getlist.
+    eauto.
+    eauto. intro; auto.
+    erewrite <- eq_env_P_getlist.
+    eauto.
+    eauto. intro; auto.
+  Qed.    
 
 
   
@@ -1966,15 +2615,25 @@ Lemma preord_env_P_def_funs_compat_pre_vals_set S k B  rho1 rho2 B' e1 e2 S1 :
     preord_exp pr cenv k (c |[ e1 ]|, rho1) (c |[ e2 ]|, rho2).
   Proof.
     intros.
-    eapply preord_exp_compat_vals_set with (S := FromList xs); eauto.
-    intros. apply H; eauto.
-    erewrite <- eq_env_P_getlist.
-    eauto.
-    eauto. intro; auto.
-    erewrite <- eq_env_P_getlist.
-    eauto.
-    eauto. intro; auto.
+    eapply preord_exp_compat_stem_vals_le; eauto.
+    eapply Disjoint_Included_l; eauto.
+    apply bound_stem_var.
   Qed.    
+
+    Corollary preord_exp_compat_stem_vals xs vs vs' k rho1 rho2 c e1 e2 :
+    (forall k rho1 rho2, preord_env_P pr cenv (occurs_free e1) k rho1 rho2 ->
+                         getlist xs rho1 = Some vs ->
+                         getlist xs rho2 = Some vs' -> 
+                         preord_exp pr cenv k (e1, rho1) (e2, rho2)) ->
+    Disjoint var (bound_stem_ctx c) (FromList xs) ->
+    getlist xs rho1 = Some vs ->
+    getlist xs rho2 = Some vs' -> 
+    preord_env_P pr cenv (occurs_free (c |[ e1 ]|)) k rho1 rho2 ->
+    preord_exp pr cenv k (c |[ e1 ]|, rho1) (c |[ e2 ]|, rho2).
+  Proof.
+    intros.
+    eapply preord_exp_compat_stem_vals_le; eauto.
+  Qed.
 
 
   (* generalization of compat_vals to a list of variable
@@ -1996,6 +2655,24 @@ Lemma preord_env_P_def_funs_compat_pre_vals_set S k B  rho1 rho2 B' e1 e2 S1 :
   Qed.
 
 
+      Corollary preord_exp_compat_stem_val x k val rho1 rho2 c e1 e2 :
+    (forall k rho1 rho2, preord_env_P pr cenv (occurs_free e1) k rho1 rho2 ->
+                         M.get x rho1 = Some val ->                         
+                         preord_exp pr cenv k (e1, rho1) (e2, rho2)) ->
+    ~ bound_stem_ctx c x ->
+    M.get x rho1 = Some val ->  
+    preord_env_P pr cenv (occurs_free (c |[ e1 ]|)) k rho1 rho2 ->
+    preord_exp pr cenv k (c |[ e1 ]|, rho1) (c |[ e2 ]|, rho2).
+  Proof.
+    intros.
+    eapply preord_exp_compat_vals_stem_set with (S := Singleton _ x); auto.
+    intros.
+    apply H. auto. specialize (H5 x). rewrite <- H1.
+    symmetry. apply H5.
+    constructor.
+    split. intro. intro. apply H0.
+    inv H3. inv H5. auto.
+  Qed.
 
     Corollary preord_exp_compat_val x k val rho1 rho2 c e1 e2 :
     (forall k rho1 rho2, preord_env_P pr cenv (occurs_free e1) k rho1 rho2 ->
@@ -2005,16 +2682,11 @@ Lemma preord_env_P_def_funs_compat_pre_vals_set S k B  rho1 rho2 B' e1 e2 S1 :
     M.get x rho1 = Some val ->  
     preord_env_P pr cenv (occurs_free (c |[ e1 ]|)) k rho1 rho2 ->
     preord_exp pr cenv k (c |[ e1 ]|, rho1) (c |[ e2 ]|, rho2).
-  Proof.
-    intros.
-    eapply preord_exp_compat_vals_set with (S := Singleton _ x); auto.
-    intros.
-    apply H. auto. specialize (H5 x). rewrite <- H1.
-    symmetry. apply H5.
-    constructor.
-    split. intro. intro. apply H0.
-    inv H3. inv H5. auto.
-Qed.
+    Proof.
+     intros. eapply preord_exp_compat_stem_val; eauto.
+     intro; apply H0.
+     apply bound_stem_var. auto.
+    Qed.
   
   
 
@@ -2065,17 +2737,17 @@ Qed.
   Qed.
     
     
-  
+   
   Theorem rw_case_equiv: forall cl c0 e x c ys rho1 rho2 k,
       findtag cl c0 = Some e ->
-      ~bound_var_ctx c x ->
+      ~bound_stem_ctx c x ->
       preord_env_P pr cenv (occurs_free (Econstr x c0 ys (c |[ Ecase x cl ]|))) k rho1 rho2 ->
       preord_exp pr cenv k (Econstr x c0 ys (c |[ Ecase x cl ]|), rho1) (Econstr x c0 ys (c |[ e ]|), rho2). 
   Proof.
     intros; intro; intros. inversion H3; subst.
     assert (Hl : Included var (FromList ys) (occurs_free (Econstr x c0 ys (c |[ Ecase x cl ]|)))).  rewrite occurs_free_Econstr. left; auto.
     assert (H11' := preord_env_P_getlist_l _ _ _ _ _ _ _ _ H1 Hl H11). destructAll.
-    eapply preord_exp_compat_val in H13; eauto.
+    eapply preord_exp_compat_stem_val in H13; eauto.
     destructAll.
     eexists. eexists.
     split. eapply BStep_constr; eauto. auto.
@@ -2109,8 +2781,34 @@ Qed.
   Definition rename_fds_clos x y :=clos_refl_trans fundefs (rename_fds_glob x y).
 
 
+  (* alternative def. of rename_clos which only admits unshadowed renames *)
+  Inductive rename_glob_s: var -> var -> exp -> exp -> Prop :=
+  | Ctx_rs: forall x y e e' c,
+      rename_loc x y e e' ->
+      ~ bound_stem_ctx c x -> 
+    rename_glob_s x y (c|[e ]|) (c|[e']|).
+
+  Inductive rename_fds_glob_s: var -> var -> fundefs -> fundefs -> Prop :=
+  | Ctx_fds_rs: forall x y e e' f,
+      rename_loc x y e e' ->
+      ~ bound_stem_fundefs_ctx f x ->
+                 rename_fds_glob_s x y (f <[ e ]>) (f <[ e' ]>).
   
-  
+  Definition rename_clos_s x y := clos_refl_trans exp (rename_glob_s x y).
+  Definition rename_fds_clos_s x y :=clos_refl_trans fundefs (rename_fds_glob_s x y).
+
+
+  Theorem rename_clos_s_included:
+    forall x y e e',
+      rename_clos_s x y e e' ->
+      rename_clos x y e e'.
+  Proof.
+    intros. induction H.
+    - inv H. constructor. constructor. auto.
+    - apply rt_refl.
+    - eapply rt_trans; eauto.
+  Qed.
+      
   Theorem rename_loc_refl_x:
     forall {x} {e e'},
     rename_loc x x e e' ->
@@ -2179,6 +2877,7 @@ Qed.
       eapply rt_trans; eauto.
   Qed.
 
+ 
 
     
   Theorem rename_context_fds_clos:
@@ -2201,6 +2900,60 @@ Qed.
       eapply rt_trans; eauto.
   Qed.
 
+
+    Theorem rename_context_clos_s:
+    forall x y e e',
+    rename_clos_s x y e e' ->      
+    forall c,
+      ~ bound_stem_ctx c x ->
+    rename_clos_s x y (c |[e ]| ) (c|[e']|).
+  Proof.
+    intros x y e e' H.
+    induction H.
+    - intro; intro.
+      inversion H; subst.
+      apply rt_step.
+      rewrite app_ctx_f_fuse.
+      rewrite app_ctx_f_fuse.
+      constructor. auto.
+      intro. apply bound_stem_comp_ctx_mut in H3.
+      inv H3; auto.      
+    - intro; intro. apply rt_refl.
+    - intro; intro.
+      specialize (IHclos_refl_trans1 c H1).
+      specialize (IHclos_refl_trans2 c H1).
+      eapply rt_trans; eauto.
+  Qed.
+
+ 
+
+    
+  Theorem rename_context_fds_clos_s:
+    forall x y e e',
+      rename_clos_s x y e e' ->
+      forall cfds,
+        ~ bound_stem_fundefs_ctx cfds x ->
+                    rename_fds_clos_s x y  (cfds <[ e ]>) (cfds <[e' ]>).
+  Proof.
+    intros x y e e' H.
+    induction H.
+    - intro; intro.
+      inversion H; subst.
+      apply rt_step.      
+      rewrite app_f_ctx_f_fuse.
+      rewrite app_f_ctx_f_fuse.
+      constructor. auto.
+      intro. apply bound_stem_comp_ctx_mut in H3.
+      inv H3; auto.      
+    - intro; intro. apply rt_refl.
+    - intro; intro.
+      specialize (IHclos_refl_trans1 cfds H1).
+      specialize (IHclos_refl_trans2 cfds H1).
+      eapply rt_trans; eauto.
+  Qed.
+
+
+  
   Section inv_app_ctx.
 
     Theorem inv_app_Hole:
@@ -2279,6 +3032,27 @@ Qed.
       eapply rt_trans; eauto.
   Qed.
 
+  Theorem rename_fds_Fcons2_s:
+    forall x y f f',
+      rename_fds_clos_s x y f f' ->
+      forall z t ys e,
+        rename_fds_clos_s x y (Fcons z t ys e f) (Fcons z t ys e f').
+  Proof.
+    intros x y f f' H.
+    induction H.
+    - inversion H; subst.
+    intros. constructor.
+    do 2 (rewrite inv_app_Fcons2).
+    constructor. auto.
+    intro. inv H2. auto.
+    - intros. apply rt_refl.
+    - intros.
+      specialize (IHclos_refl_trans1 z0 t ys e).
+      specialize (IHclos_refl_trans2 z0 t ys e).
+      eapply rt_trans; eauto.
+  Qed.
+
+  
 Theorem rename_fds_Efun:
       forall x y f f',
       rename_fds_clos x y f f' ->
@@ -2301,6 +3075,47 @@ Proof.
       eapply rt_trans; eauto.
 Qed.
 
+Theorem name_in_fundefs_clos_s:
+  forall x y z f f',
+  rename_fds_clos_s x y f f' ->
+  ~ name_in_fundefs f z ->
+  ~ name_in_fundefs f' z.
+Proof.
+  intros. induction H.
+  - inv H.
+    intro. apply H0.
+    apply name_in_fundefs_ctx_ctx. apply name_in_fundefs_ctx_ctx in H. auto.
+  - auto.
+  - eauto.
+Qed.
+
+Theorem rename_fds_Efun_s:
+      forall x y f f',
+        rename_fds_clos_s x y f f' ->
+        ~ name_in_fundefs f x ->
+      forall e,
+        rename_clos_s x y (Efun f e) (Efun f' e).
+Proof.
+    intros x y f f' H.
+    induction H.
+    - intro.
+      inv H.
+      constructor.
+      do 2 (rewrite inv_app_Efun2).
+      constructor.
+      auto.
+      intro. inv H.
+      apply H0. apply name_in_fundefs_ctx_ctx. auto.
+      auto.      
+    - intro; intro.
+      apply rt_refl.
+    - intro; intro.
+      specialize (IHclos_refl_trans1 H1 e).
+      eapply rt_trans.
+      eauto. apply IHclos_refl_trans2.
+      eapply name_in_fundefs_clos_s. apply H. auto.
+Qed.
+
 
 
 Theorem apply_r_list_end: forall x y l,
@@ -2318,8 +3133,8 @@ Qed.
 
 
 
-Lemma rename_clos_constr_l': forall x y v p e l' l ,
-                                rename_clos x y (Econstr v p (l++l') e) (Econstr v p (l++(apply_r_list (M.set x y (M.empty var)) l')) e).
+Lemma rename_clos_s_constr_l': forall x y v p e l' l ,
+                                rename_clos_s x y (Econstr v p (l++l') e) (Econstr v p (l++(apply_r_list (M.set x y (M.empty var)) l')) e).
   Proof.
     induction l'.
     - simpl. intro. apply rt_refl.
@@ -2334,6 +3149,7 @@ Lemma rename_clos_constr_l': forall x y v p e l' l ,
         rewrite  inv_app_Hole at 1.
         constructor.
         constructor.
+        intro. inv H.
         specialize (IHl' (l++[y])).
         rewrite <- app_assoc in IHl'.
         rewrite <- app_assoc in IHl'.
@@ -2347,14 +3163,14 @@ Lemma rename_clos_constr_l': forall x y v p e l' l ,
         simpl in IHl'. apply IHl'.
   Qed.
 
-  Theorem rename_clos_constr_l: forall x y v p e l ,
-                                rename_clos x y (Econstr v p l e) (Econstr v p (apply_r_list (M.set x y (M.empty var)) l) e).
+  Theorem rename_clos_s_constr_l: forall x y v p e l ,
+                                rename_clos_s x y (Econstr v p l e) (Econstr v p (apply_r_list (M.set x y (M.empty var)) l) e).
   Proof.
-    intros. apply rename_clos_constr_l' with (l := nil).
+    intros. apply rename_clos_s_constr_l' with (l := nil).
   Qed.
   
-Theorem rename_clos_prim_l': forall x y v p e l' l,
-                                rename_clos x y (Eprim v p (l++l') e) (Eprim v p (l++(apply_r_list (M.set x y (M.empty var)) l')) e).
+Theorem rename_clos_s_prim_l': forall x y v p e l' l,
+                                rename_clos_s x y (Eprim v p (l++l') e) (Eprim v p (l++(apply_r_list (M.set x y (M.empty var)) l')) e).
   Proof.
     induction l'.
     - simpl. intro. apply rt_refl.
@@ -2369,6 +3185,7 @@ Theorem rename_clos_prim_l': forall x y v p e l' l,
         rewrite  inv_app_Hole at 1.
         constructor.
         constructor.
+        intro. inv H.
         specialize (IHl' (l++[y])).
         rewrite <- app_assoc in IHl'.
         rewrite <- app_assoc in IHl'.
@@ -2382,15 +3199,15 @@ Theorem rename_clos_prim_l': forall x y v p e l' l,
         simpl in IHl'. apply IHl'.
   Qed.
 
-  Theorem rename_clos_prim_l: forall x y v p e  l,
-                                rename_clos x y (Eprim v p l e) (Eprim v p (apply_r_list (M.set x y (M.empty var)) l) e).
+  Theorem rename_clos_s_prim_l: forall x y v p e  l,
+                                rename_clos_s x y (Eprim v p l e) (Eprim v p (apply_r_list (M.set x y (M.empty var)) l) e).
 Proof.    
   intros.
-  apply rename_clos_prim_l' with (l := nil).
+  apply rename_clos_s_prim_l' with (l := nil).
 Qed.
 
-Theorem rename_clos_app_l': forall x y f c l' l,
-                                rename_clos x y (Eapp f c (l++l')) (Eapp f c (l++(apply_r_list (M.set x y (M.empty var)) l'))).
+Theorem rename_clos_s_app_l': forall x y f c l' l,
+                                rename_clos_s x y (Eapp f c (l++l')) (Eapp f c (l++(apply_r_list (M.set x y (M.empty var)) l'))).
   Proof.
     induction l'.
     - simpl. intro. apply rt_refl.
@@ -2405,6 +3222,7 @@ Theorem rename_clos_app_l': forall x y f c l' l,
         rewrite  inv_app_Hole at 1.
         constructor.
         constructor.
+        intro. inv H.
         specialize (IHl' (l++[y])).
         rewrite <- app_assoc in IHl'.
         rewrite <- app_assoc in IHl'.
@@ -2418,11 +3236,11 @@ Theorem rename_clos_app_l': forall x y f c l' l,
         simpl in IHl'. apply IHl'.
   Qed.
 
-Theorem rename_clos_app_l: forall x y f c  l,
-                                rename_clos x y (Eapp f c l) (Eapp f c (apply_r_list (M.set x y (M.empty var)) l)).
+Theorem rename_clos_s_app_l: forall x y f c  l,
+                                rename_clos_s x y (Eapp f c l) (Eapp f c (apply_r_list (M.set x y (M.empty var)) l)).
 Proof.  
   intros.
-  apply rename_clos_app_l' with (l := nil).
+  apply rename_clos_s_app_l' with (l := nil).
 Qed.  
 
 Theorem rename_clos_is_case_r: forall x y r y0,
@@ -2517,6 +3335,55 @@ Proof.
     apply IHclos_refl_trans2; auto.
 Qed.
 
+Theorem rename_clos_s_case_l: forall x y r r' ,
+                              rename_clos_s x y r r' ->
+                              forall v v' l l',
+                              r = (Ecase v l) ->
+                              r' = (Ecase v' l') ->
+                              forall a c e,
+  rename_clos_s x y
+    (Ecase a ((c, e) :: l))
+    (Ecase a ((c, e) :: l')).
+Proof.
+  intros x y r r' H.
+  induction H; intros; subst.
+  - inversion H; subst.
+    destruct c0; try inv H0.
+    + simpl in *. subst.
+      inv H4.
+      apply rt_refl.
+    + 
+      assert  (Ecase_c a ((c,e)::l0) c0 c1 l1 |[ e' ]| = Ecase a ((c,e)::l')).
+      {
+        simpl.
+        simpl in H1.
+        inv H1.
+        reflexivity.
+      }
+      rewrite <- H0.
+      replace ((c, e) :: l0 ++ (c0, c1 |[ e0 ]|) :: l1) with (((c, e) :: l0) ++ (c0, c1 |[ e0 ]|) :: l1).      
+      rewrite inv_app_Ecase.
+      rewrite app_ctx_f_fuse.
+      simpl comp_ctx_f.
+      apply rt_step.
+      constructor. auto.
+      intro. apply H5. inv H2. constructor; auto.
+      reflexivity.
+  - inv H0. apply rt_refl.
+  - assert (H0' := H0).
+    apply rename_clos_s_included in H0'. 
+    eapply rename_clos_is_case_l in H0'. 
+    Focus 2.
+    eauto.
+    destructAll.        
+    specialize (IHclos_refl_trans2 x0 v' x1 l'). 
+    specialize (IHclos_refl_trans1 v x0 l x1).
+    eapply rt_trans.
+    apply IHclos_refl_trans1; auto.
+    apply IHclos_refl_trans2; auto.
+Qed.
+
+
 
 Theorem rename_clos_case: forall (v a x y:var) l c e e' l',
   rename_clos x y (Ecase v l) (Ecase v l') ->
@@ -2533,6 +3400,25 @@ Proof.
   apply H0.
   simpl.
   eapply rename_clos_case_l.
+  apply H. reflexivity. reflexivity.
+Qed.
+
+Theorem rename_clos_s_case: forall (v a x y:var) l c e e' l',
+  rename_clos_s x y (Ecase v l) (Ecase v l') ->
+  rename_clos_s x y e e' ->  
+  rename_clos_s x y
+    (Ecase a ((c, e) :: l))
+    (Ecase a ((c, e') :: l')).
+Proof.
+  intros.
+  eapply rt_trans.
+  replace ((c,e)::l) with ([] ++ (c,e)::l) by auto.
+  rewrite inv_app_Ecase.
+  apply rename_context_clos_s.
+  apply H0.
+  intro. inv H1. inv H8.
+  simpl.
+  eapply rename_clos_s_case_l.
   apply H. reflexivity. reflexivity.
 Qed.
 
@@ -2573,6 +3459,46 @@ Proof.
     apply IHclos_refl_trans1; auto.
     apply IHclos_refl_trans2. reflexivity.
 Qed.
+
+Theorem rename_case_one_step_s:
+  forall x y r r',
+    rename_clos_s x y r r' ->
+    forall v v' l l',
+      r = (Ecase v l) ->
+      r' = (Ecase v' l') ->
+      forall a, 
+      rename_clos_s x y (Ecase a l) (Ecase a l').
+Proof.
+  intros x y r r' H.
+  induction H; intros.
+  - subst.
+    inv H.
+    destruct c; inv H0.
+    + simpl in *; subst.
+      inv H4. apply rt_refl.
+    + simpl in H1. inv H1.
+      rewrite inv_app_Ecase.
+      rewrite inv_app_Ecase.
+      apply rt_step.
+      rewrite app_ctx_f_fuse.
+      rewrite app_ctx_f_fuse.
+      constructor. apply H4.
+      intro. apply H5. constructor. inv H; auto.
+  -   subst. inv H0. apply rt_refl.
+  - subst.
+    assert (H0' := H0).
+    apply rename_clos_s_included in H0'. 
+    eapply rename_clos_is_case_l in H0'.
+    2: reflexivity.
+    destruct H0'. destruct H1.
+    subst.
+    specialize (IHclos_refl_trans2 x0 v' x1 l' eq_refl eq_refl).
+    specialize (IHclos_refl_trans1 v x0 l x1 eq_refl eq_refl).
+    eapply rt_trans.
+    apply IHclos_refl_trans1; auto.
+    apply IHclos_refl_trans2. 
+Qed.
+
 
 Theorem apply_r_none:
   forall v sigma,
@@ -2817,7 +3743,8 @@ Proof.
       auto.
     + rewrite apply_r_set2 by auto.
       assert (apply_r sigma v0 <> x).
-      unfold apply_r. destruct (@M.get M.elt v0 sigma) eqn:gv0s.
+      unfold apply_r. 
+      destruct (@M.get M.elt v0 sigma) eqn:gv0s.
       intro; subst. apply H0; eauto.
       auto.
       rewrite apply_r_set2 by auto.
@@ -3346,49 +4273,76 @@ Proof.
   - etransitivity; eauto.
 Qed.    
 
-      
+Theorem rename_glob_loc:
+  forall x y e e',
+   rename_loc x y e e' ->
+   rename_glob x y e e'. 
+Proof.
+  intros.
+  rewrite inv_app_Hole.
+  rewrite inv_app_Hole with (e := e).
+  constructor; auto.
+Qed.
 
-  Transparent rename.
+Theorem rename_glob_s_loc:
+  forall x y e e',
+   rename_loc x y e e' ->
+   rename_glob_s x y e e'. 
+Proof.
+  intros.
+  rewrite inv_app_Hole.
+  rewrite inv_app_Hole with (e := e).
+  constructor; auto. intro. inv H0.
+Qed.
+ About rename_all_fun. 
+
+Transparent rename.
   Theorem rename_corresp: forall y x,
                             (forall e,
-                               Disjoint _ (bound_var e) (FromList [x;y]) ->
-                               rename_clos x y e (rename y x e)) /\
+                               Disjoint _ (bound_var e) (FromList [y]) ->
+                               rename_clos_s x y e (rename y x e)) /\
                             (forall fds,
-                               Disjoint _ (bound_var_fundefs fds) (FromList [x;y]) ->
-                               rename_fds_clos x y fds (rename_all_fun (M.set x y (M.empty var)) fds)).
+                                Disjoint _ (bound_var_fundefs fds) (FromList [y]) ->
+                                ~ name_in_fundefs fds x ->
+                               rename_fds_clos_s x y fds (rename_all_fun (M.set x y (M.empty var)) fds)).
   Proof.
     intros y x. eapply exp_def_mutual_ind; intros; simpl.
     -  unfold rename.
       simpl.
       eapply rt_trans.
-      apply rename_clos_constr_l.
-      do 2 (rewrite inv_app_Econstr).
-      apply rename_context_clos.
-      rewrite bound_var_Econstr in H0.
-      assert (Hde := Disjoint_Union_l _ _ _ H0).
-      apply H in Hde.
-      erewrite (proj1 prop_rename_all).
-      apply Hde.
-      eapply smg_trans.
-      apply remove_set_2.
-      intro.
-      inv H0.
-      specialize (H2 x).
-      apply H2.
-      split.
-      right; auto.
-      constructor; auto.
-      apply proper_set.
-      apply remove_empty.
+      apply rename_clos_s_constr_l.      
+
+      destruct (var_dec v x).
+       + subst.         
+         replace (rename_all (M.remove x (M.set x y (M.empty var))) e) with (rename_all (M.empty var) e).
+         rewrite <- (proj1 rename_all_empty).
+         apply rt_refl.
+         auto.
+         apply prop_rename_all.
+         eapply smg_sym.
+         eapply smg_trans.
+         apply remove_set_1; auto.
+         apply remove_empty.
+       + do 2 (rewrite inv_app_Econstr).
+         apply rename_context_clos_s.                  
+         replace (rename_all (M.remove v (M.set x y (M.empty var))) e) with (rename_all (M.set x y (M.empty var)) e).
+         apply H; auto.
+         rewrite bound_var_Econstr in H0.
+         assert (Hde := Disjoint_Union_l _ _ _ H0). auto.      
+         apply prop_rename_all.
+         apply smg_sym.
+         apply remove_none.
+         rewrite M.gso; auto. apply M.gempty.
+         intro. inv H1; auto. inv H7.
     - unfold rename. simpl. unfold apply_r.
       destruct (var_dec v x).
       + subst. rewrite M.gss. apply rt_step.
         rewrite inv_app_Hole.
       rewrite inv_app_Hole at 1.
       constructor.
-      constructor. 
-      + rewrite M.gso. rewrite M.gempty. apply rt_refl. auto.
-        
+      constructor.
+      intro. inv H0.
+      + rewrite M.gso. rewrite M.gempty. apply rt_refl. auto.        
     - rewrite bound_var_Ecase_cons in H1.
       assert (Hde := Disjoint_Union_l _ _ _ H1).
       assert (Hdv := Disjoint_Union_r _ _ _ H1).
@@ -3402,12 +4356,12 @@ Qed.
       subst. rewrite M.gss. constructor.
       rewrite inv_app_Hole.
       rewrite inv_app_Hole at 1.
-      constructor. constructor.
+      constructor. constructor. intro. inv H2. 
       rewrite M.gso by auto. rewrite M.gempty.
       apply rt_refl.      
-      eapply rename_clos_case.
+      eapply rename_clos_s_case.
       unfold rename in H0. simpl in H0.
-      eapply rename_case_one_step.        
+      eapply rename_case_one_step_s.        
       apply H0. reflexivity. reflexivity.         
       apply H. 
     - unfold rename.
@@ -3415,69 +4369,80 @@ Qed.
       rewrite bound_var_Eproj in H0.      
       assert (Hde := Disjoint_Union_l _ _ _ H0).
       assert (Hdv := Disjoint_Union_r _ _ _ H0).
-      apply H in Hde.
-      inversion Hdv.
+      apply H in Hde; auto.     
+      apply rt_trans with (y := (Eproj v t n (apply_r (M.set x y (M.empty var)) v0) e)).
+      unfold apply_r. destruct (var_dec v0 x).
+      subst. rewrite M.gss. apply rt_step.
+      apply rename_glob_s_loc. constructor.
+      rewrite M.gso; auto. rewrite M.gempty. apply rt_refl.
       destruct (var_dec v x).
-      exfalso. specialize (H1 v).
-      apply H1.
-      subst. split; auto. constructor. auto.
-      eapply rt_trans.
-      Focus 2.
-      assert (map_get_r var (M.remove v (M.set x y (M.empty var))) (M.set x y (M.empty var))).
-      eapply smg_trans.
-      apply remove_set_2; eauto.
-      apply proper_set.
-      apply remove_empty.
-      assert (Hpr := prop_rename_all).
-      destruct Hpr.
-      erewrite (H3 _ _ _ H2).
-      rewrite inv_app_Eproj.
-      apply rename_context_clos.
-      apply Hde.
-      destruct (var_dec x v0).
-      + subst. 
-      unfold apply_r. rewrite M.gss.
-      simpl.
-      
-      rewrite inv_app_Hole.
-      rewrite inv_app_Hole at 1.
-      apply rt_step.
-      constructor. constructor.
-      + unfold apply_r. rewrite M.gso by auto. rewrite M.gempty.
+      + subst.
+        replace (rename_all (M.remove x (M.set x y (M.empty var))) e) with e. 
         apply rt_refl.
+        etransitivity.
+        apply rename_all_empty.
+        apply prop_rename_all. apply smg_sym.
+        eapply smg_trans.
+        apply remove_set_1; auto.
+        apply remove_empty.
+      +  replace (rename_all (M.remove v (M.set x y (M.empty var))) e) with (rename_all (M.set x y (M.empty var)) e).
+         rewrite inv_app_Eproj.
+         rewrite inv_app_Eproj.
+         apply rename_context_clos_s.
+         apply H; auto.
+         apply (Disjoint_Union_l _ _ _ H0).
+         intro. inv H1. auto. inv H8.
+         apply prop_rename_all.
+         apply smg_sym.
+         eapply smg_trans.
+         apply remove_set_2; auto.
+         apply proper_set.
+         apply remove_empty.
     - unfold rename. simpl.
       rewrite bound_var_Efun in H1.
       assert (Hdf := (Disjoint_Union_l _ _ _ H1)).
       assert (Hde := Disjoint_Union_r _ _ _ H1).
       specialize (H Hdf).
       specialize (H0 Hde).
-      eapply rt_trans.
-      rewrite inv_app_Efun1.
-      apply rename_context_clos.
-      eauto.
-      simpl.
-      erewrite (proj1 prop_rename_all).
-      Focus 2.
-      eapply smg_trans.
-      apply remove_all_not_in. intro. inversion Hdf. specialize (H3 x). apply H3.
-      split.
-      apply name_in_fundefs_bound_var_fundefs.
-      apply name_fds_same. auto.
-      constructor. auto.
-      apply proper_set.
-      apply remove_all_empty.
-      apply rename_fds_Efun.
-      erewrite (proj2 prop_rename_all).
-      apply H.
-      eapply smg_trans.
-      apply remove_all_not_in. intro.
-      inversion Hdf. specialize (H3 x). apply H3.
-      split.
-      apply name_in_fundefs_bound_var_fundefs.
-      apply name_fds_same. auto.      
-      constructor. auto.
-      apply proper_set.
-      apply remove_all_empty.
+      assert (Hf2 := Decidable_name_in_fundefs f2).
+      inv Hf2. specialize (Dec x). inv Dec.
+      + assert (map_get_r var (remove_all (M.set x y (M.empty var)) (all_fun_name f2)) (M.empty var)).
+        eapply smg_trans.
+        apply remove_all_in. apply same_name_in_fun. auto.
+        apply remove_all_empty.
+        replace (rename_all_fun (remove_all (M.set x y (M.empty var)) (all_fun_name f2)) f2) with f2.
+        replace (rename_all (remove_all (M.set x y (M.empty var)) (all_fun_name f2)) e) with e.
+        apply rt_refl.
+        etransitivity. apply rename_all_empty. symmetry.
+        eapply prop_rename_all.
+        apply H3.
+        etransitivity. apply rename_all_empty. symmetry.
+        eapply prop_rename_all.
+        apply H3.
+      + assert (map_get_r var (remove_all (M.set x y (M.empty var)) (all_fun_name f2)) (M.set x y (M.empty var))).
+        {
+          eapply smg_trans.
+          apply remove_all_not_in.
+          intro; apply H2.
+          apply same_name_in_fun; auto.
+          apply proper_set. apply remove_all_empty.
+        }
+        replace  (rename_all (remove_all (M.set x y (M.empty var)) (all_fun_name f2)) e) with
+            (rename_all (M.set x y (M.empty var)) e).        
+        
+        rewrite inv_app_Efun1.
+        eapply rt_trans.        
+        apply rename_context_clos_s.
+        apply H0.
+        intro. inv H4. auto. inv H8.
+        apply rename_fds_Efun_s.
+        replace (rename_all_fun (remove_all (M.set x y (M.empty var)) (all_fun_name f2)) f2) with
+            (rename_all_fun (M.set x y (M.empty var)) f2). apply H.
+        auto.
+        symmetry.
+        apply prop_rename_all; auto. auto.
+        symmetry.
+        apply prop_rename_all; auto.
     - unfold rename. simpl.
       unfold apply_r.
       destruct (var_dec x v).
@@ -3487,39 +4452,38 @@ Qed.
         apply rt_step.
         rewrite inv_app_Hole at 1.
         constructor. constructor.
-        simpl.
-        apply rename_clos_app_l.
+        simpl. intro. inv H0.
+        apply rename_clos_s_app_l.
       + rewrite M.gso by auto.
         rewrite M.gempty.
-        apply rename_clos_app_l.
+        apply rename_clos_s_app_l.
     - unfold rename.
       simpl.
       eapply rt_trans.
-      apply rename_clos_prim_l.
-      do 2 (rewrite inv_app_Eprim).
-      apply rename_context_clos.
-      rewrite bound_var_Eprim in H0.
-      assert (Hde := Disjoint_Union_l _ _ _ H0).
-      apply H in Hde.
-      erewrite (proj1 prop_rename_all).
-      apply Hde.
-      eapply smg_trans.
-      apply remove_set_2.
-      intro.
-      inv H0.
-      specialize (H2 x).
-      apply H2.
-      split.
-      right; auto.
-      constructor; auto.
-      apply proper_set.
-      apply remove_empty.
+      apply rename_clos_s_prim_l.
+      destruct (var_dec x v). subst.
+      + replace  (rename_all (M.remove v (M.set v y (M.empty var))) e) with e.
+        apply rt_refl.
+        etransitivity.
+        apply rename_all_empty.
+        symmetry. apply prop_rename_all.
+        eapply smg_trans. apply remove_set_1. apply remove_empty.
+      + do 2 (rewrite inv_app_Eprim).
+        apply rename_context_clos_s.
+        replace (rename_all (M.remove v (M.set x y (M.empty var))) e) with (rename_all (M.set x y (M.empty var)) e).      
+        rewrite bound_var_Eprim in H0.
+        assert (Hde := Disjoint_Union_l _ _ _ H0).
+        apply H; auto.
+        apply prop_rename_all.
+        apply smg_sym. eapply smg_trans. apply remove_set_2; auto.
+        apply proper_set. apply remove_empty.
+        intro. inv H1. auto. inv H7.
     - unfold rename.
       simpl. unfold apply_r. destruct (var_dec x v).
       subst. rewrite M.gss. constructor.
       rewrite inv_app_Hole.
       rewrite inv_app_Hole at 1.
-      constructor; constructor.
+      constructor. constructor. intro. inv H0.
       rewrite M.gso by auto.
       rewrite M.gempty.
       apply rt_refl.
@@ -3532,20 +4496,28 @@ Qed.
       assert (Hdee := Disjoint_Union_l _ _ _ Hdef5).
       apply H0 in Hdf5.
       apply H in Hdee.
-      eapply rt_trans.
-      rewrite inv_app_Fcons1.
-      eapply rename_context_fds_clos.
-      apply Hdee.      
-      simpl.
-      erewrite (proj1 prop_rename_all).
-      Focus 2.
-      eapply smg_trans.
-      apply remove_all_not_in. intro. inversion Hdl. specialize (H3 x). apply H3.
-      split. apply H2. constructor. auto.
-      apply proper_set.
-      apply remove_all_empty.
-      apply rename_fds_Fcons2.
-      auto.
+      eapply rt_trans with (y :=   (Fcons v t l e (rename_all_fun (M.set x y (M.empty var)) f5))).
+      apply rename_fds_Fcons2_s. auto.       
+      assert (Hl := Decidable_FromList l).
+      inv Hl. specialize (Dec x). inv Dec.
+      + replace (rename_all (remove_all (M.set x y (M.empty var)) l) e) with e.
+        apply rt_refl.
+        etransitivity. apply rename_all_empty.
+        apply prop_rename_all.
+        apply smg_sym.
+        eapply smg_trans.
+        apply remove_all_in. auto. apply remove_all_empty.
+      + replace  (rename_all (remove_all (M.set x y (M.empty var)) l) e) with (rename y x e).
+        do 2 (rewrite inv_app_Fcons1).
+        apply rename_context_fds_clos_s. auto. intro.
+        inv H4. auto. inv H11. 
+        apply prop_rename_all.
+        apply smg_sym.
+        eapply smg_trans.
+        apply remove_all_not_in. auto.
+        apply proper_set.
+        apply remove_all_empty.
+      + intro. apply H2. constructor 2. auto.
     - apply rt_refl.
       Unshelve.
       auto.
@@ -3565,7 +4537,7 @@ Qed.
     induction l; intros.
     - simpl app.
       simpl app in H1.
-      simpl in H1. destruct (M.get x rho1) eqn:gxr.
+      simpl in H1.      destruct (M.get x rho1) eqn:gxr.
       apply H in gxr. destructAll.
       destruct (getlist l' rho1) eqn:glr.
       eapply preord_env_P_getlist_l in glr; eauto. destructAll.
@@ -3768,9 +4740,9 @@ Qed.
   
 
   Theorem rw_proj1_equiv : forall  x x' t t' ys  y e e'  c c' n k rho1 rho2,
-                             ~ bound_var_ctx c x ->
-                             ~ bound_var_ctx c y ->
-                             ~ bound_var_ctx c' x' ->
+                             ~ bound_stem_ctx c x ->
+                             ~ bound_stem_ctx c y ->
+                             ~ bound_stem_ctx c' x' ->
                              ~ bound_var_ctx c' y  ->
                              x <> y ->
                              nthN ys n = Some y -> 
@@ -3792,7 +4764,7 @@ Qed.
     assert (Hyv := getlist_nth_get _ _ _ _ _ H16 H4).
     assert (Hyv' := getlist_nth_get _ _ _ _ _ H9 H4).
     destructAll.
-    eapply preord_exp_compat_vals with (xs := x::y::nil) in H18; eauto.
+    eapply preord_exp_compat_stem_vals with (xs := x::y::nil) in H18; eauto.
     destructAll. eexists; eexists.
     split. eapply BStep_constr; eauto.
     eauto. 
@@ -3805,7 +4777,7 @@ Qed.
       assert (Hg := getlist_two H17).
       assert (Hg' := getlist_two H19).
       destructAll. rewrite H30 in H23. inv H23.      
-      eapply preord_exp_compat_vals with (xs := x'::y::nil) in H32; eauto.
+      eapply preord_exp_compat_stem_vals with (xs := x'::y::nil) in H32; eauto.
       destructAll. eexists; eexists. split.
       eapply BStep_proj.
       eauto.
@@ -3835,7 +4807,7 @@ Qed.
         inv H26.
         apply H1. auto.
         inv H23.
-        apply H2. auto.
+        apply H2. apply bound_stem_var. auto.
         inv H26.
       }
       apply preord_env_P_extend. rewrite occurs_free_Eproj in H15.
@@ -3867,51 +4839,529 @@ Qed.
 
  
   Theorem rw_proj_clos_equiv : forall  x x' t t' ys  y e e'  c n ,
-                             ~ bound_var_ctx c x ->
-                             ~ bound_var_ctx c y ->
-                             ~ bound_var e x' ->
+                             ~ bound_stem_ctx c x ->
+                             ~ bound_stem_ctx c y ->
+(*                             ~ bound_var e x' ->  *)
                              ~ bound_var e y  ->
                              x <> y ->
-                             rename_clos x' y e e' ->
+                             rename_clos_s x' y e e' ->
                              nthN ys n = Some y ->
                              forall k rho1 rho2,
                              preord_env_P pr cenv (occurs_free (Econstr x t ys (c |[ Eproj x' t' n x e ]|))) k rho1 rho2 ->
                              preord_exp pr cenv k (Econstr x t ys (c |[ Eproj x' t' n x e ]|) , rho1 )
                                         (Econstr x t ys (c |[ Eproj x' t' n x e' ]|), rho2).
-  Proof.                                                           
-    intros.
-    revert k rho1 rho2 H6.
-    induction H4.
-    - inversion H4; subst.
+  Proof.
+    intros x x' t t' ys y e e' c n Hs_cx Hs_cy Hbv_ey Hxy Hrcs Hnth k rho1 rho2 Hpreord.
+    revert k rho1 rho2 Hpreord. 
+    induction Hrcs.
+    - inversion H; subst.
       intros.
       eapply rw_proj1_equiv; eauto.
-      intro. apply H1. apply bound_var_app_ctx. left; auto.
-      intro. apply H2. apply bound_var_app_ctx. left; auto. 
-    - intros. apply preord_exp_refl. apply H6.
+      intro. apply Hbv_ey. apply bound_var_app_ctx. left; auto. 
+    - intros. apply preord_exp_refl. auto.
     - intros.
       eapply preord_exp_trans.
-      apply IHclos_refl_trans1.
+      apply IHHrcs1.
       auto.
-      auto.
-      apply H6.
+      eauto.
       intro.
-      apply IHclos_refl_trans2.
-      apply bound_var_rename in H4_.
-      intro. apply H1.
-      apply H4_. auto.
-      intro. apply H2.
-      apply bound_var_rename in H4_.
-      apply H4_. auto.
+      apply IHHrcs2.
+      apply rename_clos_s_included in Hrcs1.
+      intro. apply Hbv_ey.
+      eapply bound_var_rename; eauto.
       apply preord_env_P_refl.
   Qed.
 
+Definition Range_map {A:Type} sig:  Ensemble A:=
+  (fun x => exists y, M.get y sig = Some x).
+
+Definition Dom_map {A:Type} sig : Ensemble (M.elt):=
+  (fun x => exists (y:A), M.get x sig = Some y).
+
+Theorem Dom_map_remove {A:Type} : forall sigma v,
+  Same_set _ (Dom_map (@M.remove A v sigma))
+                        (Setminus _ (Dom_map sigma) (Singleton _ v)).
+Proof.
+  split; intros; intro; intros.
+  inv H.
+  split.
+  exists x0.
+  eapply gr_some.  
+  apply H0.
+  intro. inv H.
+  rewrite M.grs in H0; auto. inv H0.
+  inv H.
+  inv H0.
+  exists x0.
+  rewrite M.gro; auto.
+  intro; apply H1. subst.
+  constructor.
+Qed.
+
+
+(* todo: move *)
+Theorem not_in_remove_all: forall x l sigma,
+  ~ (FromList l x) ->
+  M.get x sigma = M.get x (remove_all sigma l).
+Proof.
+  induction l; intros.
+  reflexivity.
+  simpl. 
+  assert (~ (a = x) /\ ~ (FromList l x)).
+  split; intro. apply H. constructor; auto.
+  apply H. constructor 2; auto.
+  destruct H0.
+  rewrite <- IHl; auto.
+  symmetry.
+  rewrite M.gro; auto.
+Qed.  
+
+Theorem remove_all_some:
+  forall x y l sigma,
+    M.get x (remove_all sigma l) = Some y ->
+    ~ (FromList l x).
+Proof.
+  induction l.
+  intros. intro. inv H0.
+  simpl.
+  intros.
+  intro. inv H0.
+  rewrite remove_all_none in H. inv H.
+  rewrite M.grs; auto.
+  eapply IHl; eauto.
+Qed.  
+
+Theorem Dom_map_empty {A}:
+  Same_set _ (Dom_map (M.empty A)) (Empty_set _).
+Proof.
+  split; intro. intro. inv H. rewrite M.gempty in H0. inv H0.
+  intro. inv H.
+Qed.
+
+Theorem Dom_map_set:
+  forall (sig:M.t var) x y,
+    Same_set _ (Dom_map (M.set x y sig)) (Union _ [set x] (Dom_map sig)).
+Proof.
+  intros. split. intro. intro. inv H. destruct (var_dec x0 x).
+  subst; auto.
+  rewrite M.gso in H0 by auto.
+  right. exists x1; auto.
+  intro. intro. inv H. exists y. inv H0. rewrite M.gss.
+  auto.
+  destruct (var_dec x x0). subst. exists y.
+  rewrite M.gss. auto.
+  inv H0. exists x1. rewrite M.gso; auto.
+Qed.  
+
+Theorem Dom_map_set_list:
+  forall (sig: M.t var) lx ly,
+  length lx = length ly ->
+  Same_set _ (Dom_map (set_list (combine lx ly) sig)) (Union _ (FromList lx) (Dom_map sig)).
+Proof.
+  induction lx.
+  - intros. destruct ly.
+    simpl. rewrite FromList_nil. auto with Ensembles_DB.
+    inv H.
+  - intros. destruct ly; inv H.
+    simpl. rewrite FromList_cons.
+    rewrite Dom_map_set.
+    apply IHlx in H1. rewrite H1.  auto 25 with Ensembles_DB.
+Qed.    
+
+
+Theorem Dom_map_remove_all: forall l sigma ,
+  Same_set _ (Dom_map (remove_all sigma l))
+           (Setminus _ (Dom_map sigma) (FromList l)).
+Proof.
+  split; intro; intro.
+  inv H.
+  assert (~ (FromList l x)) by apply (remove_all_some _ _ _ _ H0).
+  split; auto.
+  rewrite <- not_in_remove_all in H0; auto.
+  exists x0; auto.  
+  inv H.
+  inv H0.
+  exists x0.
+  rewrite <- not_in_remove_all; auto.
+Qed.
+
+
+Theorem Range_map_remove {A:Type}: forall sigma v,
+  Included _ (Range_map (@M.remove A v sigma))
+                        (Range_map sigma).
+Proof.
+  intros. intro. intros. inv H.
+  exists x0.
+  eapply gr_some.
+  apply H0.
+Qed.
+
+Theorem Range_map_remove_all : forall l sigma ,
+  Included _ (Range_map (remove_all sigma l))
+                        (Range_map sigma).
+Proof.
+  induction l; intros.
+  simpl. reflexivity.
+  simpl. eapply Included_trans.
+  apply IHl.
+  apply Range_map_remove.
+Qed.
+
+Theorem apply_r_sigma_in:
+  forall sigma a,
+  In _ (Union _ (Setminus _ (Singleton _ a) (Dom_map sigma)) (Range_map sigma)) (apply_r sigma a).
+Proof.
+  unfold apply_r.
+  intros.
+  destruct (Maps.PTree.get a sigma) eqn:gas.
+  right. exists a. auto.
+  left.
+  split.
+  constructor.
+  intro. inv H. rewrite gas in H0. inv H0.
+Qed.  
+  
+Theorem FromList_apply_r_list:
+  forall sigma l,
+  Included _ (FromList (apply_r_list sigma l))
+           (Union _ (Setminus var (FromList l) (Dom_map sigma)) (Range_map sigma)).
+  Proof.
+    induction l.
+    - simpl. intro. intro.
+      inv H.
+    - simpl.
+      rewrite FromList_cons.
+      rewrite FromList_cons.
+      apply Union_Included.
+      intro. intros.
+      inv H.
+      assert (Hrs := apply_r_sigma_in sigma a).
+      inv Hrs. left.
+      inv H.
+      split; auto.
+      right; auto.
+      intro; intro.
+      apply IHl in H.
+      inv H.
+      left. inv H0.
+      split; auto.
+      right; auto.
+  Qed.
+
+  Theorem Dom_map_setlist: forall xs vs,
+    Included _  (Dom_map (set_list (combine xs vs) (M.empty var)))
+                (FromList xs).
+  Proof.
+    induction xs.
+    - intros.
+      simpl.
+      intro. intro. inv H.
+      rewrite M.gempty in H0. inv H0.
+    - intro. simpl. destruct vs. simpl.
+      intro. intro. inv H.
+      rewrite M.gempty in H0. inv H0.
+      simpl.
+      rewrite FromList_cons.
+      intro. intro.
+      destruct (var_dec a x).
+      subst. left; auto.
+      right.
+      specialize (IHxs vs).
+      apply IHxs.
+      inv H. rewrite M.gso in H0 by auto.
+      exists x0.
+      apply H0.
+  Qed.      
+
+  Theorem Dom_map_setlist_ss: forall xs vs,
+                             length xs = length vs -> 
+    Same_set _  (Dom_map (set_list (combine xs vs) (M.empty var)))
+                (FromList xs).
+  Proof.
+    induction xs.
+    - intros. split.
+      simpl.
+      intro. intro. inv H.
+      inv H0. 
+      rewrite M.gempty in H. inv H.
+      intro. intro. inv H0.
+    - intros. simpl. simpl in H. destruct vs.
+      inv H.
+      simpl in H.
+      inv H. apply IHxs in H1.
+      split.
+      intro. intro. inv H.
+      rewrite FromList_cons.
+      simpl in H0.
+      destruct (var_dec a x).
+      subst. left; auto.
+      right.
+      apply H1.
+      rewrite M.gso in H0 by auto.
+      exists x0.
+      apply H0.
+      intro. intros.
+      destruct (var_dec a x).
+      subst.
+      simpl. exists v. apply M.gss.
+      inv H.
+      exfalso; auto.
+      apply H1 in H0. simpl.
+      inv H0.
+      exists x0. rewrite M.gso; auto.
+  Qed.      
+
+  
+  Theorem Range_map_setlist: forall xs vs, 
+    Included _  (Range_map (set_list (combine xs vs) (M.empty var)))
+                (FromList vs).
+  Proof.
+    induction xs; intros.
+    - simpl. intro.
+      intro. inv H. rewrite M.gempty in H0. inv H0.
+    - simpl. specialize IHxs. destruct vs. simpl.
+      intro; intro; inv H. rewrite M.gempty in H0. inv H0.
+      simpl.
+      rewrite FromList_cons.
+      intro. intro.
+      inv H. destruct (var_dec x0 a).
+      subst.      
+      rewrite M.gss in H0.
+      left. inv H0.
+      constructor.
+      right. 
+      apply IHxs.
+      rewrite M.gso in H0 by auto.
+      exists x0. auto.
+Qed.
+
+  (* todo: move to identifiers? *)
+Theorem name_not_free_in_fds: 
+forall fds, Disjoint var (occurs_free_fundefs fds) (name_in_fundefs fds).
+Proof.
+  induction fds.
+  - simpl. rewrite occurs_free_fundefs_Fcons.
+    eauto 25 with Ensembles_DB.
+  - simpl. eauto with Ensembles_DB.
+Qed.
+
+
+Theorem of_rename_all_mut: 
+(forall e sigma, (occurs_free (rename_all sigma e)) \subset
+                                    Union _ (Setminus _ (occurs_free e) (Dom_map sigma)) (Range_map sigma))
+/\
+(forall fds sigma, (occurs_free_fundefs (rename_all_fun sigma fds)) \subset
+                                    Union _ (Setminus _ (occurs_free_fundefs fds) (Dom_map sigma)) (Range_map sigma)).
+Proof.
+  apply exp_def_mutual_ind; intros.
+  - simpl.
+    repeat normalize_occurs_free.
+    apply Union_Included.
+    + eapply Included_trans.
+      apply FromList_apply_r_list.
+      eauto with Ensembles_DB.
+    + apply Setminus_Included_Included_Union.
+      eapply Included_trans.
+      apply H.
+      assert (Hd := Dom_map_remove sigma v).
+      assert (Hr := Range_map_remove sigma v).
+      intro.
+      intros. inv H0.
+      destruct (var_dec x v).
+      * subst. right. constructor.
+      * inv H1.
+        left. left. split.
+        right. split; auto.
+        intro. apply n; inv H1.
+        auto.
+        intro.
+        apply H2.
+        inv H1.
+        exists x0.
+        rewrite M.gro by auto. auto.
+      * apply Hr in H1.
+        eauto.        
+  - simpl.
+    repeat normalize_occurs_free.
+    intro. intros.
+    inv H.
+    apply apply_r_sigma_in.
+  - simpl.
+    repeat normalize_occurs_free.
+    specialize (H sigma).
+    specialize (H0 sigma).
+    repeat (apply Union_Included).
+    + eapply Included_trans.
+      intro; intro.
+      inv H1.
+      apply apply_r_sigma_in.
+      eauto with Ensembles_DB.
+    + eapply Included_trans.
+      apply H.
+      eauto with Ensembles_DB.
+    + eapply Included_trans.
+      apply H0.
+      eauto with Ensembles_DB.
+  - simpl.
+    repeat normalize_occurs_free.
+        apply Union_Included.
+    + eapply Included_trans.
+      intro. intro. inv H0.
+      apply apply_r_sigma_in.
+      eauto with Ensembles_DB.
+    + apply Setminus_Included_Included_Union.
+      eapply Included_trans.
+      apply H.
+      assert (Hd := @Dom_map_remove var sigma v).
+      assert (Hr := Range_map_remove sigma v).
+      intro.
+      intros. inv H0.
+      destruct (var_dec x v).
+      * subst. right. constructor.
+      * inv H1.
+        left. left. split.
+        right. split; auto.
+        intro. apply n0; inv H1.
+        auto.
+        intro.
+        apply H2.
+        inv H1.
+        exists x0.
+        rewrite M.gro by auto. auto.
+      * apply Hr in H1.
+        eauto.
+  - simpl.
+    repeat normalize_occurs_free.
+    apply Union_Included.
+    + eapply Included_trans.
+      apply H.
+      apply Union_Included.
+      * intro.  intro. inv H1.
+        left. split. left.  auto.
+        intro.
+        apply H3.
+        apply Dom_map_remove_all.
+        split. auto.
+        assert (Hnf := name_not_free_in_fds).
+        specialize (Hnf f2).
+        inv Hnf. specialize (H4 x). intro; apply H4.
+        split; auto.
+        apply name_fds_same.
+        auto.        
+      * right.
+        eapply Range_map_remove_all.
+        apply H1.
+    + apply Setminus_Included_Included_Union.
+      eapply Included_trans.
+      apply H0.
+      apply Union_Included.
+      * intro. intro.
+        inv H1.
+        assert (Hh := Decidable_name_in_fundefs f2).
+        inv Hh. specialize (Dec x).
+        destruct Dec.
+        right. apply rename_all_fun_name. auto.       
+        left.  left. split. right. split; auto.
+        intro; apply H3. 
+        apply Dom_map_remove_all.
+        split; auto.
+        intro; apply H1.
+        apply name_fds_same. auto.
+      * left; right.
+        eapply Range_map_remove_all. apply H1.
+  - simpl.
+    repeat normalize_occurs_free.
+    apply Union_Included.
+    eapply Included_trans.
+    apply FromList_apply_r_list.
+    eauto with Ensembles_DB.
+    eapply Included_trans.
+    intro. intro. inv H.
+    apply apply_r_sigma_in.
+    eauto with Ensembles_DB.
+  -  simpl.
+    repeat normalize_occurs_free.
+        apply Union_Included.
+    + eapply Included_trans.
+      apply FromList_apply_r_list.
+      eauto with Ensembles_DB.
+    + apply Setminus_Included_Included_Union.
+      eapply Included_trans.
+      apply H.
+      assert (Hd := Dom_map_remove sigma v).
+      assert (Hr := Range_map_remove sigma v).
+      intro.
+      intros. inv H0.
+      destruct (var_dec x v).
+      * subst. right. constructor.
+      * inv H1.
+        left. left. split.
+        right. split; auto.
+        intro. apply n; inv H1.
+        auto.
+        intro.
+        apply H2.
+        inv H1.
+        exists x0.
+        rewrite M.gro by auto. auto.
+      * apply Hr in H1.
+        eauto.
+  - simpl.
+    rewrite occurs_free_Ehalt.
+    rewrite occurs_free_Ehalt.
+    intro. intro. inv H. apply apply_r_sigma_in.
+  - simpl.
+    repeat normalize_occurs_free.
+    apply Union_Included.
+    + intro. intro. inv H1. apply H in H2.
+      inv H2.
+      left. inv H1.
+      split.
+      left. split; auto.
+      intro.
+      inv H1. apply H3; auto.
+      rewrite rename_all_fun_name in H3.
+      apply H3; auto.
+      intro; apply H4.
+      apply Dom_map_remove_all.
+      split. auto.
+      intro; apply H3; auto.      
+      right.
+      eapply Range_map_remove_all.
+      apply H1.
+    + intro. intro. inv H1.
+      apply H0 in H2.
+      inv H2.
+      inv H1. left.
+      split; auto.
+      right. split; auto.
+      auto.
+  - simpl.
+    intro. intro. inv H.
+Qed.
+
+
+Corollary rename_not_occurs_free:
+  forall e a fb,
+    e <> a ->
+    Disjoint var (occurs_free (rename e a fb)) [set a].
+Proof.
+  intros.
+  eapply Disjoint_Included_l.
+  apply of_rename_all_mut.
+  split. intro. intro. inv H0. inv H2. inv H1.
+  - inv H0. apply H2.
+    rewrite Dom_map_set. auto.
+  - inv H0. destruct (var_dec x0 x).
+    subst. rewrite M.gss in H1. inv H1. auto.
+    rewrite M.gso in H1 by auto. rewrite M.gempty in H1. inv H1.
+Qed.
 
   
   (* rw rule for proj *)
   Corollary rw_proj_equiv : forall  x x' t t' ys  y e c n k rho1 rho2,
-                             ~ bound_var_ctx c x ->
-                             ~ bound_var_ctx c y ->
-                             ~ bound_var e x' ->
+                             ~ bound_stem_ctx c x ->
+                             ~ bound_stem_ctx c y ->
                              ~ bound_var e y  ->
                              x <> y ->
                              x' <> y ->
@@ -3921,14 +5371,12 @@ Qed.
                                         (Econstr x t ys (c |[ rename y x' e ]|), rho2).
   Proof.                                                           
     intros.
-    assert (rename_clos x' y e (rename y x' e)).
+    assert (rename_clos_s x' y e (rename y x' e)).
     apply rename_corresp.
     split.
     intros.
-    intro. inversion H7. inv H9.
-    auto.
-    inv H11. auto.
-    inversion H9.
+    intro. inversion H6. subst. inv H8. auto.
+    inv H9.
     eapply preord_exp_trans.
     eapply rw_proj_clos_equiv; eauto.
     intros.
@@ -3936,16 +5384,13 @@ Qed.
     do 2 (rewrite app_ctx_f_fuse). 
     apply preord_exp_compat.
     intros.
-    assert (num_occur (rename y x' e) x' 0).
-    apply rename_dead_var. auto.
-    split. intro. intro. apply H1. 
-    inv H9. inv H11.
-    auto.
     apply rm_proj.
-    auto.
+    assert (y <> x') by auto.
+    apply rename_not_occurs_free with (fb := e) in H8.  intro. inv H8. specialize (H10 x').
+    apply H10. split; auto with Ensembles_DB.
     2: apply preord_env_P_refl.
     eapply preord_env_P_antimon.
-    apply H8.
+    apply H7.
     apply reflexivity.
   Qed.
 
@@ -4077,13 +5522,13 @@ Qed.
                                        eq_env_P (Union _ (occurs_free_fundefs fl) (name_in_fundefs fl)) (def_funs fl fl rho2 rho2) rho2' ->
                                        preord_exp pr cenv k' (e, rho1') (e', rho2')) ->
     preord_env_P pr cenv (occurs_free (Efun fl (c|[e]|))) k rho1 rho2 ->
-    Disjoint var (bound_var_ctx c) (occurs_free_fundefs fl)  ->
-    Disjoint var (bound_var_ctx c) (name_in_fundefs fl)  -> 
+    Disjoint var (bound_stem_ctx c) (occurs_free_fundefs fl)  ->
+    Disjoint var (bound_stem_ctx c) (name_in_fundefs fl)  -> 
     preord_exp pr cenv k (Efun fl (c |[ e ]|) , rho1) (Efun fl (c|[ e' ]|), rho2).
 Proof.
   intros. intro. intros.
   inv H4.
-  eapply preord_exp_compat_vals_set in H10; eauto.
+  eapply preord_exp_compat_vals_stem_set in H10; eauto.
   destructAll.
   eexists. eexists.
   split.
@@ -4096,7 +5541,60 @@ Proof.
   apply H0.
 Qed.
 
-(* could make that more general like rename_loc_equiv *)
+(* shadowed version of preord_rename_clos *)
+Theorem preord_rename_clos_s: forall fb fb' v a e t,
+  (Disjoint _ (bound_var fb) (Singleton _ e)) ->
+  rename_clos_s a e fb fb' ->
+  M.get e (M.set a v t) = Some v ->
+ forall k, 
+  preord_exp pr cenv k (fb, M.set a v t) (fb', M.set a v t).
+Proof.
+  intros fb fb' v a e t Hde Hrc Hg.
+  induction Hrc.
+  - intros.
+    destruct (var_dec a e). subst.
+    inv H.
+    apply rename_loc_refl_x in H0. subst.
+    apply preord_exp_refl. apply preord_env_P_refl.
+    inv H.
+    assert ( getlist [a; e] (M.set a v t) = Some (v::v::nil)).
+    simpl. rewrite M.gss. rewrite Hg.  reflexivity.
+    eapply preord_exp_compat_stem_vals with (xs := a::e::nil); eauto.
+    intros.
+    eapply rename_loc_equiv; eauto.
+    intro. intros. simpl in H3.  simpl in H4.
+    destruct (M.get a rho1).
+    destruct (M.get e rho1).
+    inv H3. 
+    inv H5.
+    destruct (M.get a rho2).
+    destruct (M.get e rho2).
+    inv H4. exists v1. split.
+    reflexivity.
+    apply preord_val_refl.
+    inv H4.
+    inv H4.
+    inv H3.
+    inv H3.    
+    split. intro. intro. inv H2. inv H4.
+    auto. inv H2. inv Hde.
+    specialize (H2 x). apply H2.
+    split; auto. rewrite bound_var_app_ctx; auto.
+    left. apply bound_stem_var. auto.
+    inv H4.
+    apply preord_env_P_refl.
+  - intros. apply preord_exp_refl. apply preord_env_P_refl.
+  - intros.
+    eapply preord_exp_trans.
+    apply IHHrc1. auto.
+    intro.
+    apply IHHrc2.
+    apply rename_clos_s_included in Hrc1. 
+    apply bound_var_rename in Hrc1.
+    rewrite <- Hrc1. auto.
+Qed.
+
+
 Theorem preord_rename_clos: forall fb fb' v a e t,
   (Disjoint _ (bound_var fb) (Singleton _ a)) ->
   (Disjoint _ (bound_var fb) (Singleton _ e)) ->
@@ -4258,13 +5756,15 @@ Proof.
       apply H. exists x; auto.
 Qed.    
 
+
+
+(* setlist_rename_all now without Disjoint _ (bound_var fb) (FromList xs) *)
 Theorem setlist_rename_all:
   forall xs ys vs rho2 rho2',
     NoDup xs ->
     getlist ys rho2 = Some vs ->
     setlist xs vs rho2 = Some rho2'  ->
     forall fb,
-      (Disjoint _ (bound_var fb) (FromList xs)) ->
       (Disjoint _ (bound_var fb) (FromList ys)) ->
     (Disjoint _ (FromList ys) (FromList xs)) ->
     forall k,
@@ -4272,17 +5772,17 @@ Theorem setlist_rename_all:
                (rename_all (set_list (combine xs ys) (M.empty var)) fb, rho2).
 Proof.
   induction xs; intros ys vs rho2 rho2' Nb; intros.
-  - inv H0. destruct vs; inv H5.
+  - inv H0. destruct vs; inv H4.
     rewrite <- (proj1 rename_all_empty).
     apply preord_exp_refl. apply preord_env_P_refl.    
   - assert (length (a::xs) = length vs).
     eapply setlist_length_eq. apply H0.
-    destruct vs; simpl in H4.
-    inv H4.
+    destruct vs; simpl in H3.
+    inv H3.
     simpl in H0.
     assert (length ys = length (v::vs)).
     eapply getlist_length_eq. apply H.
-    destruct ys; simpl in H3. inv H5.
+    destruct ys; simpl in H3. inv H4.
     simpl in H.
     destruct (M.get e rho2) eqn:ger2.
     destruct (getlist ys rho2) eqn:glyr2.
@@ -4293,34 +5793,21 @@ Proof.
     simpl set_list.
     inv H.
     inversion Nb; subst.
-    specialize (IHxs _ _ _ _  H8 glyr2 slxr2).
-    clear H7 H8.
+    specialize (IHxs _ _ _ _  H7 glyr2 slxr2).
+    clear H7 H6.
     inv H0.
     
-    assert (rename_clos a e fb (rename e a fb)).
+    assert (rename_clos_s a e fb (rename e a fb)).
     {
       apply (proj1 (rename_corresp e a)).
-      split.
-      intro.
-      intro.
-      inv H.
-      inv H6.
-      inv H1. specialize (H x). apply H.
-      split; auto.
-      constructor. auto.
-      inv H.
-      inv H2.
-      specialize (H x). apply H.
-      split. auto. constructor; auto.
-      inv H6.
+      eapply Disjoint_Included_r; eauto.
+      intro. intro. constructor. inv H. auto.
+      inv H0.
     }            
     eapply preord_exp_trans.
-    eapply preord_exp_trans.    
-    eapply preord_rename_clos.
-    3: apply H.
+    eapply preord_exp_trans.
+    eapply preord_rename_clos_s. 2: apply H.     
     eapply Disjoint_FromList_r. apply H1.
-    constructor; auto.
-    eapply Disjoint_FromList_r. apply H2.
     constructor; auto.
     destruct (var_dec e a). subst.
     rewrite M.gss. auto. 
@@ -4328,26 +5815,21 @@ Proof.
     erewrite <- setlist_not_In.
     apply ger2.
     apply slxr2.
-    intro. inv H3.
-    specialize (H6 e).
-    apply H6.
+    intro. inv H2. 
+    specialize (H5 e).
+    apply H5.
     split. constructor. auto.
     constructor 2. apply H0.
-    intros.    
-    apply rm_set.
-    assert (e <> a).
-    intro. subst.
-    inv H3. specialize (H0 a).
-    apply H0.
-    split; auto. constructor; auto.
-    constructor; auto.    
-    apply (proj1 (rename_dead_var e a H0)).
-    eapply Disjoint_FromList_r. apply H1. constructor; auto.
+    intros.
+    assert (e <> a). intro. inv H2. specialize (H5 a). apply H5; split; constructor; auto.
+    eapply preord_exp_refl.
+    apply preord_env_P_set_not_in_P_l.
+    apply preord_env_P_refl.
+    apply rename_not_occurs_free. auto.
     intro.
     eapply preord_exp_trans.
     apply IHxs.
-    rewrite <- bound_var_rename; eauto.
-    eapply Disjoint_FromList_cons. eauto.
+    apply rename_clos_s_included in H. 
     rewrite <- bound_var_rename; eauto.
     eapply Disjoint_FromList_cons. eauto.    
     eapply Disjoint_FromList_cons.
@@ -4362,23 +5844,13 @@ Proof.
     apply preord_env_P_refl.
     apply setlist_empty_not_in.
     intro.
-    inv H3. specialize (H6 e).
-    apply H6. split; auto.
+    inv H2. specialize (H5 e).
+    apply H5. split; auto.
     constructor; auto.
     constructor 2; auto.
 Qed.
 
 
-
-(* todo: move to identifiers? *)
-Theorem name_not_free_in_fds: 
-forall fds, Disjoint var (occurs_free_fundefs fds) (name_in_fundefs fds).
-Proof.
-  induction fds.
-  - simpl. rewrite occurs_free_fundefs_Fcons.
-    eauto 25 with Ensembles_DB.
-  - simpl. eauto with Ensembles_DB.
-Qed.
 Theorem Disjoint_bindings_find_def: forall f t xs fb fds,
  unique_bindings_fundefs fds ->
   find_def f fds = Some (t, xs, fb) ->
@@ -4421,17 +5893,18 @@ Proof.
       inv H0. intro.
       apply H3. left. auto.
   -   intros. inv H.
-Qed.  
+Qed.
 
 
+(* Main lemma for function inlining *)
 Theorem rw_fun_corr:
   forall f fds t xs fb vs c rho1 rho2 k,
   find_def f fds = Some (t, xs, fb) ->
-  (* lot of these can be reduces to unique_binding and closed top level *)
+  (* next few can be deduced from unique_binding and closed top level *)
   Disjoint _ (Union _ (FromList xs) (bound_var fb)) (FromList vs) ->
-  unique_bindings_fundefs fds -> 
-  Disjoint var (bound_var_ctx c) (occurs_free_fundefs fds)  ->
-  Disjoint var (bound_var_ctx c) (bound_var_fundefs fds)  -> 
+  unique_name_fundefs fds -> 
+  Disjoint var (bound_stem_ctx c) (occurs_free_fundefs fds)  ->
+  Disjoint var (bound_stem_ctx c) (name_in_fundefs fds)  -> 
   List.NoDup xs ->
   preord_env_P pr cenv (occurs_free (Efun fds (c |[ Eapp f t vs ]|))) k rho1 rho2 ->
   preord_exp pr cenv k (Efun fds (c |[ Eapp f t vs ]|), rho1)
@@ -4439,7 +5912,7 @@ Theorem rw_fun_corr:
 Proof.
   intros f fds t xs fb vs c rho1 rho2 k H H0 Hub H1 H2 H3 H4.
   apply fun_inline_compat_clos; auto.
-  (* probably want this compat clos to also show that fds is already bound to the right thing in rho2' *)
+  (* probably want this compat clos to also show that fds is already bound to the right things in rho2' *)
   intros.
 
   destruct k'.
@@ -4487,7 +5960,6 @@ Proof.
   Focus 2.
   intro.
   eapply setlist_rename_all; eauto.
-  eapply Disjoint_bindings_find_def; eauto.
   
   eapply Disjoint_Included_l; eauto. right. auto.
   apply Disjoint_sym.
@@ -4512,16 +5984,13 @@ Proof.
   left; auto.
   apply name_not_free_in_fds.
 
-
+ (* fb =~ fb w/o def_funs fds*) 
   intro.
   apply preord_exp_refl.
   eapply preord_env_P_setlist_l with (P1 := Setminus _ (occurs_free fb) (FromList xs)).
   5: apply H14.
   4: apply H13.
   Focus 3. apply Forall2_refl. apply preord_val_refl.
-  Focus 3. eapply Disjoint_Included_r.
-  apply name_in_fundefs_bound_var_fundefs.
-  auto.
   Focus 2. intros. split; auto.
   eapply preord_env_P_trans.
   {
@@ -4550,6 +6019,8 @@ Proof.
     split; auto.
   }  
 Qed.
+
+
   
 
 (* can be restricted to bound_var on the path to hole in c *)
@@ -4710,7 +6181,7 @@ Proof with now eauto.
       apply rm_proj; auto.
     + apply preord_exp_compat; auto. 
       intros.
-      apply rm_fundefs; auto.
+      apply rm_fundefs_of; auto.
     + eapply preord_exp_compat; auto.
       intros.
       eapply rm_any_fundefs; auto.
@@ -4725,55 +6196,6 @@ Proof with now eauto.
       intros.
       
       apply rw_fun_corr; auto.
-      {
-        split. intro; intro. inv H4.
-        
-        (* check if x is bound in c0 *)
-        assert (Hof := Decidable_occurs_free (c0 |[ Eapp f t vs ]|)).
-        inv Hof. specialize (Dec x). 
-        rewrite occurs_free_Efun in H2. rewrite bound_var_Efun in H2.
-        destruct Dec.
-        + inv H2. specialize (H7 x).
-          apply H7.
-          split. right.          
-          split. apply H4.
-          intro. inv H.
-          assert (Hdj := Disjoint_bindings_fundefs _ _ _ _ _ H11 H3). inv Hdj.
-          specialize (H x). apply H. split; auto.
-          left.
-          inv H5.
-          eapply name_boundvar_arg. apply H2.
-          apply H3.
-          eapply bv_in_find_def. 
-          apply H3.
-          auto. 
-        + assert (bound_var_ctx c0 x).
-                   
-          eapply occurs_free_app_bound_var.
-          2: apply H4. constructor. auto.
-          inv H. inv H12. specialize (H x).
-          apply H. split.
-          rewrite bound_var_app_ctx. left; auto.
-          inv H5.
-          eapply name_boundvar_arg. apply H8.
-          apply H3.
-          eapply bv_in_find_def. 
-          apply H3.
-          auto.
-      }
-      inv H. auto.
-      apply Disjoint_sym.
-      eapply Disjoint_Included_l.
-      2: eapply Disjoint_Included_r.
-      3: apply H2.
-      rewrite occurs_free_Efun. left; auto.
-      rewrite bound_var_Efun. right. apply bound_var_app_ctx. left; auto.
-      inv H. eapply Disjoint_Included_l.
-      2: apply H8.
-      intro. intros. apply bound_var_app_ctx.
-      left; auto.
-      inv H.
-      eapply ub_find_def_nodup; eauto.
   - apply preord_exp_refl; auto.
   - eapply preord_exp_trans; eauto.
     intros.
@@ -5330,467 +6752,8 @@ Qed.
 
 
 
-Definition Range_map {A:Type} sig:  Ensemble A:=
-  (fun x => exists y, M.get y sig = Some x).
-
-Definition Dom_map {A:Type} sig : Ensemble (M.elt):=
-  (fun x => exists (y:A), M.get x sig = Some y).
-
-Theorem Dom_map_remove {A:Type} : forall sigma v,
-  Same_set _ (Dom_map (@M.remove A v sigma))
-                        (Setminus _ (Dom_map sigma) (Singleton _ v)).
-Proof.
-  split; intros; intro; intros.
-  inv H.
-  split.
-  exists x0.
-  eapply gr_some.  
-  apply H0.
-  intro. inv H.
-  rewrite M.grs in H0; auto. inv H0.
-  inv H.
-  inv H0.
-  exists x0.
-  rewrite M.gro; auto.
-  intro; apply H1. subst.
-  constructor.
-Qed.
-
-
-(* todo: move *)
-Theorem not_in_remove_all: forall x l sigma,
-  ~ (FromList l x) ->
-  M.get x sigma = M.get x (remove_all sigma l).
-Proof.
-  induction l; intros.
-  reflexivity.
-  simpl. 
-  assert (~ (a = x) /\ ~ (FromList l x)).
-  split; intro. apply H. constructor; auto.
-  apply H. constructor 2; auto.
-  destruct H0.
-  rewrite <- IHl; auto.
-  symmetry.
-  rewrite M.gro; auto.
-Qed.  
-
-Theorem remove_all_some:
-  forall x y l sigma,
-    M.get x (remove_all sigma l) = Some y ->
-    ~ (FromList l x).
-Proof.
-  induction l.
-  intros. intro. inv H0.
-  simpl.
-  intros.
-  intro. inv H0.
-  rewrite remove_all_none in H. inv H.
-  rewrite M.grs; auto.
-  eapply IHl; eauto.
-Qed.  
-
-Theorem Dom_map_empty {A}:
-  Same_set _ (Dom_map (M.empty A)) (Empty_set _).
-Proof.
-  split; intro. intro. inv H. rewrite M.gempty in H0. inv H0.
-  intro. inv H.
-Qed.
-
-Theorem Dom_map_set:
-  forall (sig:M.t var) x y,
-    Same_set _ (Dom_map (M.set x y sig)) (Union _ [set x] (Dom_map sig)).
-Proof.
-  intros. split. intro. intro. inv H. destruct (var_dec x0 x).
-  subst; auto.
-  rewrite M.gso in H0 by auto.
-  right. exists x1; auto.
-  intro. intro. inv H. exists y. inv H0. rewrite M.gss.
-  auto.
-  destruct (var_dec x x0). subst. exists y.
-  rewrite M.gss. auto.
-  inv H0. exists x1. rewrite M.gso; auto.
-Qed.  
-
-Theorem Dom_map_set_list:
-  forall (sig: M.t var) lx ly,
-  length lx = length ly ->
-  Same_set _ (Dom_map (set_list (combine lx ly) sig)) (Union _ (FromList lx) (Dom_map sig)).
-Proof.
-  induction lx.
-  - intros. destruct ly.
-    simpl. rewrite FromList_nil. auto with Ensembles_DB.
-    inv H.
-  - intros. destruct ly; inv H.
-    simpl. rewrite FromList_cons.
-    rewrite Dom_map_set.
-    apply IHlx in H1. rewrite H1.  auto 25 with Ensembles_DB.
-Qed.    
-
-
-Theorem Dom_map_remove_all: forall l sigma ,
-  Same_set _ (Dom_map (remove_all sigma l))
-           (Setminus _ (Dom_map sigma) (FromList l)).
-Proof.
-  split; intro; intro.
-  inv H.
-  assert (~ (FromList l x)) by apply (remove_all_some _ _ _ _ H0).
-  split; auto.
-  rewrite <- not_in_remove_all in H0; auto.
-  exists x0; auto.  
-  inv H.
-  inv H0.
-  exists x0.
-  rewrite <- not_in_remove_all; auto.
-Qed.
-
-
-Theorem Range_map_remove {A:Type}: forall sigma v,
-  Included _ (Range_map (@M.remove A v sigma))
-                        (Range_map sigma).
-Proof.
-  intros. intro. intros. inv H.
-  exists x0.
-  eapply gr_some.
-  apply H0.
-Qed.
-
-Theorem Range_map_remove_all : forall l sigma ,
-  Included _ (Range_map (remove_all sigma l))
-                        (Range_map sigma).
-Proof.
-  induction l; intros.
-  simpl. reflexivity.
-  simpl. eapply Included_trans.
-  apply IHl.
-  apply Range_map_remove.
-Qed.
-
-
-
-Theorem apply_r_sigma_in:
-  forall sigma a,
-  In _ (Union _ (Setminus _ (Singleton _ a) (Dom_map sigma)) (Range_map sigma)) (apply_r sigma a).
-Proof.
-  unfold apply_r.
-  intros.
-  destruct (@M.get M.elt a sigma) eqn:gas.
-  right. exists a.
-  auto.
-  left.
-  split.
-  constructor.
-  intro. inv H. rewrite gas in H0. inv H0.
-Qed.  
+    
   
-Theorem FromList_apply_r_list:
-  forall sigma l,
-  Included _ (FromList (apply_r_list sigma l))
-           (Union _ (Setminus var (FromList l) (Dom_map sigma)) (Range_map sigma)).
-  Proof.
-    induction l.
-    - simpl. intro. intro.
-      inv H.
-    - simpl.
-      rewrite FromList_cons.
-      rewrite FromList_cons.
-      apply Union_Included.
-      intro. intros.
-      inv H.
-      assert (Hrs := apply_r_sigma_in sigma a).
-      inv Hrs. left.
-      inv H.
-      split; auto.
-      right; auto.
-      intro; intro.
-      apply IHl in H.
-      inv H.
-      left. inv H0.
-      split; auto.
-      right; auto.
-  Qed.
-
-  Theorem Dom_map_setlist: forall xs vs,
-    Included _  (Dom_map (set_list (combine xs vs) (M.empty var)))
-                (FromList xs).
-  Proof.
-    induction xs.
-    - intros.
-      simpl.
-      intro. intro. inv H.
-      rewrite M.gempty in H0. inv H0.
-    - intro. simpl. destruct vs. simpl.
-      intro. intro. inv H.
-      rewrite M.gempty in H0. inv H0.
-      simpl.
-      rewrite FromList_cons.
-      intro. intro.
-      destruct (var_dec a x).
-      subst. left; auto.
-      right.
-      specialize (IHxs vs).
-      apply IHxs.
-      inv H. rewrite M.gso in H0 by auto.
-      exists x0.
-      apply H0.
-  Qed.      
-
-  Theorem Dom_map_setlist_ss: forall xs vs,
-                             length xs = length vs -> 
-    Same_set _  (Dom_map (set_list (combine xs vs) (M.empty var)))
-                (FromList xs).
-  Proof.
-    induction xs.
-    - intros. split.
-      simpl.
-      intro. intro. inv H.
-      inv H0. 
-      rewrite M.gempty in H. inv H.
-      intro. intro. inv H0.
-    - intros. simpl. simpl in H. destruct vs.
-      inv H.
-      simpl in H.
-      inv H. apply IHxs in H1.
-      split.
-      intro. intro. inv H.
-      rewrite FromList_cons.
-      simpl in H0.
-      destruct (var_dec a x).
-      subst. left; auto.
-      right.
-      apply H1.
-      rewrite M.gso in H0 by auto.
-      exists x0.
-      apply H0.
-      intro. intros.
-      destruct (var_dec a x).
-      subst.
-      simpl. exists v. apply M.gss.
-      inv H.
-      exfalso; auto.
-      apply H1 in H0. simpl.
-      inv H0.
-      exists x0. rewrite M.gso; auto.
-  Qed.      
-
-  
-  Theorem Range_map_setlist: forall xs vs, 
-    Included _  (Range_map (set_list (combine xs vs) (M.empty var)))
-                (FromList vs).
-  Proof.
-    induction xs; intros.
-    - simpl. intro.
-      intro. inv H. rewrite M.gempty in H0. inv H0.
-    - simpl. specialize IHxs. destruct vs. simpl.
-      intro; intro; inv H. rewrite M.gempty in H0. inv H0.
-      simpl.
-      rewrite FromList_cons.
-      intro. intro.
-      inv H. destruct (var_dec x0 a).
-      subst.      
-      rewrite M.gss in H0.
-      left. inv H0.
-      constructor.
-      right. 
-      apply IHxs.
-      rewrite M.gso in H0 by auto.
-      exists x0. auto.
-Qed.
-      
-
-Theorem of_rename_all_mut: 
-(forall e sigma, (occurs_free (rename_all sigma e)) \subset
-                                    Union _ (Setminus _ (occurs_free e) (Dom_map sigma)) (Range_map sigma))
-/\
-(forall fds sigma, (occurs_free_fundefs (rename_all_fun sigma fds)) \subset
-                                    Union _ (Setminus _ (occurs_free_fundefs fds) (Dom_map sigma)) (Range_map sigma)).
-Proof.
-  apply exp_def_mutual_ind; intros.
-  - simpl.
-    repeat normalize_occurs_free.
-    apply Union_Included.
-    + eapply Included_trans.
-      apply FromList_apply_r_list.
-      eauto with Ensembles_DB.
-    + apply Setminus_Included_Included_Union.
-      eapply Included_trans.
-      apply H.
-      assert (Hd := Dom_map_remove sigma v).
-      assert (Hr := Range_map_remove sigma v).
-      intro.
-      intros. inv H0.
-      destruct (var_dec x v).
-      * subst. right. constructor.
-      * inv H1.
-        left. left. split.
-        right. split; auto.
-        intro. apply n; inv H1.
-        auto.
-        intro.
-        apply H2.
-        inv H1.
-        exists x0.
-        rewrite M.gro by auto. auto.
-      * apply Hr in H1.
-        eauto.        
-  - simpl.
-    repeat normalize_occurs_free.
-    intro. intros.
-    inv H.
-    apply apply_r_sigma_in.
-  - simpl.
-    repeat normalize_occurs_free.
-    specialize (H sigma).
-    specialize (H0 sigma).
-    repeat (apply Union_Included).
-    + eapply Included_trans.
-      intro; intro.
-      inv H1.
-      apply apply_r_sigma_in.
-      eauto with Ensembles_DB.
-    + eapply Included_trans.
-      apply H.
-      eauto with Ensembles_DB.
-    + eapply Included_trans.
-      apply H0.
-      eauto with Ensembles_DB.
-  - simpl.
-    repeat normalize_occurs_free.
-        apply Union_Included.
-    + eapply Included_trans.
-      intro. intro. inv H0.
-      apply apply_r_sigma_in.
-      eauto with Ensembles_DB.
-    + apply Setminus_Included_Included_Union.
-      eapply Included_trans.
-      apply H.
-      assert (Hd := @Dom_map_remove var sigma v).
-      assert (Hr := Range_map_remove sigma v).
-      intro.
-      intros. inv H0.
-      destruct (var_dec x v).
-      * subst. right. constructor.
-      * inv H1.
-        left. left. split.
-        right. split; auto.
-        intro. apply n0; inv H1.
-        auto.
-        intro.
-        apply H2.
-        inv H1.
-        exists x0.
-        rewrite M.gro by auto. auto.
-      * apply Hr in H1.
-        eauto.
-  - simpl.
-    repeat normalize_occurs_free.
-    apply Union_Included.
-    + eapply Included_trans.
-      apply H.
-      apply Union_Included.
-      * intro.  intro. inv H1.
-        left. split. left.  auto.
-        intro.
-        apply H3.
-        apply Dom_map_remove_all.
-        split. auto.
-        assert (Hnf := name_not_free_in_fds).
-        specialize (Hnf f2).
-        inv Hnf. specialize (H4 x). intro; apply H4.
-        split; auto.
-        apply name_fds_same.
-        auto.        
-      * right.
-        eapply Range_map_remove_all.
-        apply H1.
-    + apply Setminus_Included_Included_Union.
-      eapply Included_trans.
-      apply H0.
-      apply Union_Included.
-      * intro. intro.
-        inv H1.
-        assert (Hh := Decidable_name_in_fundefs f2).
-        inv Hh. specialize (Dec x).
-        destruct Dec.
-        right. apply rename_all_fun_name. auto.       
-        left.  left. split. right. split; auto.
-        intro; apply H3. 
-        apply Dom_map_remove_all.
-        split; auto.
-        intro; apply H1.
-        apply name_fds_same. auto.
-      * left; right.
-        eapply Range_map_remove_all. apply H1.
-  - simpl.
-    repeat normalize_occurs_free.
-    apply Union_Included.
-    eapply Included_trans.
-    apply FromList_apply_r_list.
-    eauto with Ensembles_DB.
-    eapply Included_trans.
-    intro. intro. inv H.
-    apply apply_r_sigma_in.
-    eauto with Ensembles_DB.
-  -  simpl.
-    repeat normalize_occurs_free.
-        apply Union_Included.
-    + eapply Included_trans.
-      apply FromList_apply_r_list.
-      eauto with Ensembles_DB.
-    + apply Setminus_Included_Included_Union.
-      eapply Included_trans.
-      apply H.
-      assert (Hd := Dom_map_remove sigma v).
-      assert (Hr := Range_map_remove sigma v).
-      intro.
-      intros. inv H0.
-      destruct (var_dec x v).
-      * subst. right. constructor.
-      * inv H1.
-        left. left. split.
-        right. split; auto.
-        intro. apply n; inv H1.
-        auto.
-        intro.
-        apply H2.
-        inv H1.
-        exists x0.
-        rewrite M.gro by auto. auto.
-      * apply Hr in H1.
-        eauto.
-  - simpl.
-    rewrite occurs_free_Ehalt.
-    rewrite occurs_free_Ehalt.
-    intro. intro. inv H. apply apply_r_sigma_in.
-  - simpl.
-    repeat normalize_occurs_free.
-    apply Union_Included.
-    + intro. intro. inv H1. apply H in H2.
-      inv H2.
-      left. inv H1.
-      split.
-      left. split; auto.
-      intro.
-      inv H1. apply H3; auto.
-      rewrite rename_all_fun_name in H3.
-      apply H3; auto.
-      intro; apply H4.
-      apply Dom_map_remove_all.
-      split. auto.
-      intro; apply H3; auto.      
-      right.
-      eapply Range_map_remove_all.
-      apply H1.
-    + intro. intro. inv H1.
-      apply H0 in H2.
-      inv H2.
-      inv H1. left.
-      split; auto.
-      right. split; auto.
-      auto.
-  - simpl.
-    intro. intro. inv H.
-Qed.
-
 Theorem name_in_fundefs_rename_all_ns:
   forall sig f,
     name_in_fundefs f <--> name_in_fundefs (rename_all_fun_ns sig f).
@@ -6313,8 +7276,7 @@ Qed.
 End occurs_free_rw.
 
 Section Shrink_Rewrites.
-
-  
+ 
 (* shrink rewrites  *)
 Inductive sr_rw: relation exp :=
   (* Rules about dead var elimination *)
@@ -6636,6 +7598,8 @@ Qed.
     apply num_occur_rename_all_not_range_mut.
   Qed.
 
+
+  
   Theorem num_occur_rename_all_ns_not_range_mut:
     forall f sigma,
       ~ Range_map sigma f ->
@@ -7113,12 +8077,10 @@ Proof.
     split.
     eapply num_occur_n. constructor; eauto.
     assert (Hn := num_occur_arl _ _ [v] Hxy).
-    simpl in Hn. simpl. unfold var in *.
-    unfold M.elt in *.
-    omega.
+    simpl in Hn. simpl.  rewrite plus_0_r. auto. 
     eapply num_occur_n. constructor. auto.
     assert (Hnn := num_occur_set_arl _ _ Hxy [v]).
-    simpl. simpl in Hnn. unfold var in *. unfold M.elt in *. omega.
+    simpl. simpl in Hnn. do 3 (rewrite plus_0_r). rewrite plus_comm. auto.
   - inv H1; inv H2. inv H7; inv H6.
     specialize (H _ _ H8 H7).
     assert (num_occur (Ecase v l) x ( num_occur_list [v] x + m)).
@@ -7140,11 +8102,10 @@ Proof.
     split.
     eapply num_occur_n. constructor; eauto. 
     assert (Hn := num_occur_arl _ _ [v0] Hxy).
-    simpl in Hn. simpl. unfold var, M.elt in *.
-    omega.
+    simpl in Hn. simpl. rewrite plus_0_r. auto.
     eapply num_occur_n. constructor; eauto.
     assert (Hnn := num_occur_set_arl _ _ Hxy [v0]).
-    simpl. simpl in Hnn. unfold var, M.elt in *. omega.
+    simpl. simpl in Hnn. unfold var in *. unfold M.elt in *. rewrite Hnn. omega.
   - inv H1; inv H2.
     specialize (H _ _ H8 H9).
     specialize (H0 _ _ H5 H4).
@@ -7153,9 +8114,9 @@ Proof.
   - inv H; inv H0. split; eapply num_occur_n; eauto.    
     assert (Hn := num_occur_arl _ _ (v::l) Hxy).
     simpl in Hn. simpl.
-    unfold var, M.elt in *. omega.
+    unfold var in *. unfold M.elt in *. omega.
     assert (Hnn := num_occur_set_arl _ _ Hxy (v::l)).
-    simpl. simpl in Hnn. unfold var, M.elt in *. omega.
+    simpl. simpl in Hnn. unfold var in *. unfold M.elt in *. omega.
   - specialize (H _ _ H8 H7).
     destruct H.
     split; eapply num_occur_n; eauto.
@@ -7164,10 +8125,11 @@ Proof.
   - inv H; inv H0.
     split; eapply num_occur_n; eauto.
     assert (Hn := num_occur_arl _ _ [v] Hxy).
-    simpl in Hn. simpl. unfold var, M.elt in *.
+    simpl in Hn. simpl. unfold var in *.
+    unfold M.elt in *. 
     omega.
     assert (Hnn := num_occur_set_arl _ _ Hxy [v]).
-    simpl. simpl in Hnn. unfold var, M.elt in *. omega.
+    simpl. simpl in Hnn. unfold var in *.  unfold M.elt in *. omega.
   - inv H1; inv H2. specialize (H _ _ H10 H9).
     specialize (H0 _ _ H11 H12).
     destruct H; destruct H0.
@@ -7368,12 +8330,17 @@ Proof.
   intros;
   inv H1;
   inv H2;
-  try (solve [constructor; constructor; auto]).
-  -  constructor. constructor.
+  try (solve [constructor; constructor; constructor; try (apply (not_occurs_not_free)); auto]).
+  -  constructor. constructor.     
+     constructor.
+     eapply Forall_impl. 2: apply H1.
+     intros.
+     apply not_occurs_not_free. auto.
+  - do 2 (constructor).
     apply Fun_rem; auto.
     apply ub_app_ctx_f in H.
     destructAll.
-    inv H2. auto.
+    inv H2. apply unique_bind_has_unique_name.  auto. 
   -  constructor.
      constructor.
      constructor; auto.
@@ -7383,7 +8350,8 @@ Proof.
     intro.
     apply H6.
     apply bound_var_app_ctx.
-    left; auto.    
+    left.
+    apply bound_stem_var. auto.
   - constructor.
     constructor.
     assert (H' := H).
@@ -7395,7 +8363,7 @@ Proof.
     eauto with Ensembles_DB.
     constructor; auto.
     + intro; apply H6.
-      apply bound_var_app_ctx; auto.
+      apply bound_var_app_ctx. left. apply bound_stem_var; auto.
     + intro.
       destruct (bound_var_ctx_dec c).
       specialize (Dec k). inv Dec.
@@ -7403,17 +8371,17 @@ Proof.
         apply H9.
         split; auto.
         rewrite bound_var_Econstr. rewrite bound_var_app_ctx.
+        left. left. apply bound_stem_var.
         auto.
       * inv H0. specialize (H9 k).
         apply H9.
         split.
         rewrite bound_var_app_ctx.
         rewrite bound_var_Econstr.
-        rewrite bound_var_app_ctx.
-        auto.
+        rewrite bound_var_app_ctx. right. left. left.
+        apply bound_stem_var. auto.
         apply occurs_free_ctx_not_bound; auto.
         apply nthN_FromList in H1. auto.
-    + inv H4; auto.
     + destruct (bound_var_ctx_dec c).
       specialize (Dec k). inv Dec.
       * intro.
@@ -7431,7 +8399,6 @@ Proof.
         rewrite bound_var_Eproj.  auto.
         apply occurs_free_ctx_not_bound; auto.
         apply nthN_FromList in H1. auto.
-
     + intro; subst.
       (* either k is in the bv of c and H2 is false, 
             or k isn't and k is in of (since it appears in ys re:H1) *)
@@ -7473,9 +8440,6 @@ Proof.
     + constructor.    
       constructor.
       apply Fun_inline.
-      * apply ub_app_ctx_f in H. destructAll; auto.
-      * apply Disjoint_sym.
-        eapply Disjoint_bv_of_ctx; eauto.
       * erewrite find_def_fundefs_append_r. simpl.
         destruct (M.elt_eq f f). reflexivity. exfalso; auto.
         simpl.         destruct (M.elt_eq f f). reflexivity. exfalso; auto.
@@ -7490,6 +8454,99 @@ Proof.
         apply H9. split.
         apply name_in_fundefs_bound_var_fundefs. auto.
         constructor. left. auto.
+      * apply ub_app_ctx_f in H. destructAll.
+        inv H2.
+        split. intro. intro.
+        inv H2. 
+        assert (Hof := Decidable_occurs_free (c0 |[ Eapp f t vs ]|)).
+        inv Hof. specialize (Dec x). 
+        destruct Dec.
+        {
+          assert (Hnf:= Decidable_name_in_fundefs  (fundefs_append B1 (Fcons f t xs fb B2))).
+          inv Hnf. specialize (Dec x).
+          inv Dec.
+          eapply fundefs_append_unique_bindings_l in H8. 2: reflexivity.
+          destructAll.
+          eapply fundefs_append_name_in_fundefs in H10. 2: reflexivity.
+          inv H10. inv H12. specialize (H10 x).
+          apply H10. split.
+          apply name_in_fundefs_bound_var_fundefs.
+          auto.
+          apply bound_var_fundefs_Fcons. inv H5; auto.
+          inv H11.  inv H13. 
+          inv H10.
+          inv H5; auto.
+          apply name_in_fundefs_bound_var_fundefs in H10.
+          inv H5; auto. inv H21. specialize (H5 x). apply H5; auto.
+          inv H22. specialize (H5 x). apply H5; auto.
+          assert (occurs_free (Efun (fundefs_append B1 (Fcons f t xs fb B2)) (c0 |[ Eapp f t vs ]|)) x).
+          apply Free_Efun1; auto.          
+          assert (Hc := bound_var_ctx_dec c). inv Hc.
+          specialize (Dec x). inv Dec.
+          inv H4. specialize (H13 x).
+          apply H13. split. auto.
+          constructor. 
+          eapply fundefs_append_bound_vars. reflexivity.
+          right.
+          apply bound_var_fundefs_Fcons.
+          inv H5; auto.
+          assert ((occurs_free (c |[ Efun (fundefs_append B1 (Fcons f t xs fb B2)) (c0 |[ Eapp f t vs ]|) ]|) x)).          
+          apply occurs_free_ctx_not_bound; auto.
+          inv H0. specialize (H14 x).
+          apply H14. split; auto.
+          apply bound_var_app_ctx. right.
+          rewrite bound_var_Efun.
+          left.
+          eapply fundefs_append_bound_vars. reflexivity.
+          right. apply bound_var_fundefs_Fcons.
+          inv H5; auto.
+        }
+        { assert (bound_var_ctx c0 x).         
+          eapply occurs_free_app_bound_var.
+          2: apply H2. constructor. auto.          
+          inv H9. specialize (H11 x).
+          apply H11. split.
+          rewrite bound_var_app_ctx. left; auto.
+          eapply fundefs_append_bound_vars.
+          reflexivity. right.
+          rewrite bound_var_fundefs_Fcons.
+          inv H5; eauto.
+        }
+      * apply unique_bind_has_unique_name.
+        apply ub_app_ctx_f in H. destructAll.
+        inv H2.
+        auto.
+      * split; intro. intro. inv H2. 
+        assert (Hc := bound_var_ctx_dec c).        
+        inv Hc. specialize (Dec x).
+        apply ub_app_ctx_f in H. destructAll.
+        inv Dec.
+        inv H6. specialize (H8 x). apply H8. split; auto.
+        apply bound_var_Efun.
+        right. apply bound_var_app_ctx. left.
+        apply bound_stem_var; auto.
+        assert (occurs_free ( Efun (fundefs_append B1 (Fcons f t xs fb B2)) (c0 |[ Eapp f t vs ]|)) x).
+        apply Free_Efun2. auto.
+        assert (occurs_free (c |[ Efun (fundefs_append B1 (Fcons f t xs fb B2)) (c0 |[ Eapp f t vs ]|) ]|) x).
+        apply occurs_free_ctx_not_bound; auto.
+        inv H0. specialize (H10 x). apply H10. split; auto.
+        apply bound_var_app_ctx. right. apply bound_var_Efun.
+        right. apply bound_var_app_ctx. left. apply bound_stem_var; auto.
+      * apply ub_app_ctx_f in H. destructAll.
+        inv H2.
+        eapply Disjoint_Included_r.
+        apply name_in_fundefs_bound_var_fundefs.        
+        eapply Disjoint_Included_l.
+        2: apply H9.
+        etransitivity.
+        apply bound_stem_var.
+        rewrite bound_var_app_ctx.
+        apply Included_Union_l.        
+      * apply ub_app_ctx_f in H. destructAll.
+        inv H2.
+        eapply fundefs_append_unique_bindings_l in H8. 2: reflexivity.
+        destructAll.
+        inv H5; auto.
     + constructor.
       constructor.
       rewrite <- (proj1 (Disjoint_dom_rename_all_eq _)).
@@ -7500,7 +8557,9 @@ Proof.
       split. intro. intro.  inv H5. inv H16. specialize (H5 x). apply H5; auto.
       apply Fun_rem.
       * apply ub_app_ctx_f in H. destructAll.
-        inv H2; auto.
+        inv H2.
+        apply unique_bind_has_unique_name.
+        auto.
       * inv H3. 
         apply num_occur_app_ctx in H7. destructAll.
         inv H3.
